checkpoint

formal/theories/Task01/run_sim.c
@@ -1,0 +1,28 @@
+#include <stdio.h>
+#include <stdlib.h>
+#include <math.h>
+#include "state.h"
+
+StateList* run_sim(State state, double tstop, double dt) {
+
+    // Get list to accumulate results.
+    StateList* states = new_state_list();
+
+    // Main simulation loop
+    int i = 0;
+    while (state.item[TimeItem] <= tstop) {
+        // Record state.
+        state_list_append(states, state);
+
+        // Calculate derivative from current state.
+        State derivatives = diffeq(state);
+
+        // Advance state one time step
+        one_step(&state, &derivatives, dt);
+
+        // Kludge to get time showing up nicely.
+        i++;
+        state.item[TimeItem] = round(i * dt * 1.0e6) / 1.0e6;
+    }
+    return states;
+}
