formal/diguty/float_text_io.v
@@ -1,0 +1,233 @@
+(** FloatIO
+
+   Coqsim_io provides conversion operations between Coq strings
+   and the Coq/Compcert data types used in simulation.
+
+   The definitions meant for external use are:
+
+   - nl                                                        A string with a new-line character
+
+   The other definitions are in module FloatIO.
+
+   - Z_to_float (z: Z)                                         Convert Coq integer to float
+   - fraction_to_float (m d: Z)                                Convert fraction m*(10^(-d)) to float.
+   - nat_power_of_float (x: float) (n: nat)                    x^n
+   - Z_to_string_base10 (num : Z) (min_digits: nat) : string   Convert Z to string with min_digits.
+   - pad_to_width (width: nat) (s: string)                     Pad string with leading blanks up to width
+   - float_to_string (width fdigs: nat) (x: float)             Convert float to string like Ew.(fdigs-1)
+   - float_list_to_string (width fdigs: nat) (add_new_line: bool) (al : list float)
+                                                               Convert list of floats to string using
+                                                               float_to_string width fdigs, and if
+                                                               add_new_line is true, append a new line
+                                                               at the end.
+ *)
+From compcert Require Import Floats.
+Import Float.
+From compcert Require Import Fappli_IEEE.
+From compcert Require Import Integers.
+Require Import Coq.Lists.List.
+Require Import BinNums.
+Require Import Coq.QArith.QArith_base.
+Require Import Strings.String.
+Require Import Strings.Ascii.
+Require Import Coq.ZArith.Znat.
+Require Import Recdef.
+
+(** Pretty printing
+ *)
+Open Scope Z.
+Open Scope bool_scope.
+Open Scope string_scope.
+Definition nl := String "010"%char EmptyString.
+Close Scope char_scope.
+
+(* Version 8.8 has concat but earlier versions don't so include it
+   for compatibility.
+ *)
+
+(** *** Concatenating lists of strings *)
+
+(** [concat sep sl] concatenates the list of strings [sl], inserting
+    the separator string [sep] between each. *)
+
+Fixpoint concat (sep : string) (ls : list string) :=
+  match ls with
+  | nil => EmptyString
+  | cons x nil => x
+  | cons x xs => x ++ sep ++ concat sep xs
+  end.
+
+
+
+Module FloatIO.
+  (* Convert Coq integer to float *)
+  Definition Z_to_float (z: Z) :=
+    match z with
+    | Z0 => Float.zero
+    | Zpos x => from_parsed 10 x 0
+    | Zneg x => neg (from_parsed 10 x 0)
+    end.
+
+  (* Convert a decimal fraction to float.
+     First parameter, m, is an integer with all the
+     significant digits. The second
+     parameter, d, is the number of digits that
+     should follow the decimal point.
+     The resulting values is
+
+     m * (10^(-d)).
+     
+   *)
+  Definition fraction_to_float (m d: Z) :=
+    match m with
+    | Z0 => Float.zero
+    | Zpos x => from_parsed 10 x (-d)
+    | Zneg x => neg (from_parsed 10 x (-d))
+    end.
+
+  Definition floating_one := Z_to_float 1.
+
+  Fixpoint nat_power_of_float (x: float) (n: nat) : float :=
+    match n with
+    | O => floating_one
+    | S p => (mul x (nat_power_of_float x p))
+    end.
+  
+Module Details.
+  
+Definition precision_of_float := 53%Z.
+Definition log10of2scaled3 := 301.
+
+(* Compute approximate scaling exponent of 10, f, needed to
+   get a number with given binary exponent, e, in the range
+   10^(d-1) <= value < 10^d
+
+   so we can extract d significant digits.
+ *)
+Definition scale_exp (d e: Z) :=
+  d - 2 - (e + precision_of_float - 1)*log10of2scaled3/1000.
+
+Definition digits (n : Z) : string :=
+  match n with
+  | 0  => "0" | 6  => "6" | 12 => "c" | 18 => "i" | 24 => "o" | 30 => "u"
+  | 1  => "1" | 7  => "7" | 13 => "d" | 19 => "j" | 25 => "p" | 31 => "v"
+  | 2  => "2" | 8  => "8" | 14 => "e" | 20 => "k" | 26 => "q" | 32 => "w"
+  | 3  => "3" | 9  => "9" | 15 => "f" | 21 => "l" | 27 => "r" | 33 => "x"
+  | 4  => "4" | 10 => "a" | 16 => "g" | 22 => "m" | 28 => "s" | 34 => "y"
+  | 5  => "5" | 11 => "b" | 17 => "h" | 23 => "n" | 29 => "t" | 35 => "z"
+  | _  => "! Error. Max radix is 35 !"
+  end. 
+
+(* Repeat the given string n times. *)
+Fixpoint repeat_string (n: nat) (c: string) : string :=
+  match n with
+  | O => ""
+  | S x => c ++ repeat_string x c
+  end.
+
+(* Helper function when computing the digits of an integer base 10. *)
+Fixpoint Z_to_string_base10_aux (num : Z) (min_digits fuel: nat) : string :=
+  if (num <? 0) then
+    "Require non-negative num."
+  else
+    match fuel with
+    | O => "out of fuel"
+    | S x => match num with
+            | 0 => repeat_string min_digits "0"
+            | _ => (Z_to_string_base10_aux (num / 10) (pred min_digits) x) ++ digits (num mod 10)
+            end
+    end.
+
+Definition Z_to_string_base10 (num : Z) (min_digits: nat) : string :=
+  if num <? 0 then
+    "-" ++ Z_to_string_base10_aux (-num) min_digits 100
+  else
+    if (num =? 0)%Z then
+      repeat_string min_digits "0"
+    else
+      Z_to_string_base10_aux num min_digits 100.
+
+(* Convert float to Z scaled by 10**fdigs. *)
+Definition scaled_float_to_Z (x : float) (fdigs: Z) :=
+  match to_long (mul x (from_parsed 10 1 fdigs)) with
+  | Some ii => Int64.signed ii
+  | None    => 0%Z
+  end.
+
+(* Insert decimal point so there are fdigs digits after
+   the decimal point.
+ *)
+Definition insert_decimal(s: string) (fdigs: nat) :=
+  let len := length s in
+  let front := (len - fdigs)%nat in
+  (substring 0 front s) ++ "." ++ (substring front fdigs s).
+
+(* Convert positive finite float to string with given
+   number of digits of precision. Other floats return
+   empty string as they are covered by the 
+   floatToStringUnpadded function below.
+*)
+Definition float_to_string_unsigned (x: float) (fdigs: nat) :=
+  match x with
+  | B754_finite false m e _ =>
+    let digs_after_dec := pred fdigs in
+    let scale := scale_exp (Z.of_nat fdigs) e in
+    let scaled := scaled_float_to_Z x scale in
+    let b10 := Z_to_string_base10 scaled 1 in
+    let lb10 := length b10 in
+    let scale' :=
+        if (lb10 <? fdigs)%nat then
+          scale + (Z.of_nat (fdigs - lb10))
+        else
+          scale
+            in
+    let b10' :=
+        if (lb10 <? fdigs)%nat then
+          let scaled' := scaled_float_to_Z x scale' in
+          Z_to_string_base10 scaled' fdigs
+        else
+          b10
+            in
+    let d10 := insert_decimal b10' digs_after_dec in
+    let true_exp := (Z.of_nat fdigs) - scale' - 1 in
+    let exp_string := Z_to_string_base10 true_exp 1 in
+    d10 ++ "e" ++ exp_string
+  | _ => ""
+  end.
+
+Definition float_to_string_unpadded (x: float) (fdigs: nat) :=
+  match x with
+  | B754_zero false => "0.0"
+  | B754_zero true => "-0.0"
+  | B754_infinity false => "inf"
+  | B754_infinity true => "-inf"
+  | B754_nan false _ => "nan"
+  | B754_nan true _ => "-nan"
+  | B754_finite false m e _ => float_to_string_unsigned x fdigs
+  | B754_finite true m e _ => "-" ++ float_to_string_unsigned (abs x) fdigs
+  end.
+
+Definition pad_to_width (width: nat) (s: string) :=
+  let ls := length s in
+  let pads := repeat_string (width - ls) " " in
+  pads ++ s.
+
+(* Float to string in Ew.d format, with width w and digits d. *)
+Definition float_to_string (width fdigs: nat) (x: float)  :=
+  pad_to_width width (float_to_string_unpadded x fdigs).
+
+Fixpoint float_list_to_string (width fdigs: nat) (add_new_line: bool) (al : list float) : string :=
+  match al with
+  | nil => if add_new_line then nl else ""
+  | hd :: tl => (float_to_string width fdigs hd) ++ (float_list_to_string width fdigs add_new_line tl)
+  end.
+
+End Details.
+
+(* Export items from the details module that the user will want. *)
+Definition Z_to_string_base10 := Details.Z_to_string_base10.
+Definition pad_to_width := Details.pad_to_width.
+Definition float_to_string := Details.float_to_string.
+Definition float_list_to_string := Details.float_list_to_string.
+
+End FloatIO.
