formal/hash/Hashfun.v
@@ -1,0 +1,869 @@
+(** * Hashfun: Functional model of hash tables *)
+
+(** ** This C program, [hash.c], implements a hash table with
+   external chaining.  See http://www.cs.princeton.edu/~appel/HashTables.pdf
+   for an introduction to hash tables.  *)
+
+(** 
+
+#include <stddef.h>
+
+extern void * malloc (size_t n);
+extern void exit(int n);
+extern size_t strlen(const char *str);
+extern char *strcpy(char *dest, const char *src);
+extern int strcmp(const char *str1, const char *str2);
+
+unsigned int hash (char *s) {
+  unsigned int n=0;
+  unsigned int i=0;
+  int c=s[i];
+  while (c) {
+    n = n*65599u+(unsigned)c;
+    i++;
+    c=s[i];
+  }
+  return n;
+}
+
+struct cell {
+  char *key;
+  unsigned int count;
+  struct cell *next;
+};
+
+enum {N = 109};
+
+struct hashtable {
+  struct cell *buckets[N];
+};
+
+char *copy_string (char *s) {
+  int i,n = strlen(s)+1;
+  char *p = malloc(n);
+  if (!p) exit(1);
+  strcpy(p,s);
+  return p;
+}
+
+struct hashtable *new_table (void) {
+  int i;
+  struct hashtable *p = (struct hashtable * )malloc(sizeof(struct hashtable));
+  if (!p) exit(1);
+  for (i=0; i<N; i++) p->buckets[i]=NULL;
+  return p;
+}  
+
+struct cell *new_cell (char *key, int count, struct cell *next) {
+  struct cell *p = (struct cell * )malloc(sizeof(struct cell));
+  if (!p) exit(1);
+  p->key = copy_string(key);
+  p->count = count;
+  p->next = next;
+  return p;
+}
+
+unsigned int get (struct hashtable *table, char *s) {
+  unsigned int h = hash(s);
+  unsigned int b = h % N;
+  struct cell *p = table->buckets[b];
+  while (p) {
+    if (strcmp(p->key, s)==0)
+      return p->count;
+    p=p->next;
+  }
+  return 0;
+}
+
+void incr_list (struct cell **r0, char *s) {
+  struct cell *p, **r;
+  for(r=r0; ; r=&p->next) {
+    p = *r;
+    if (!p) {
+      *r = new_cell(s,1,NULL);
+      return;
+    }
+    if (strcmp(p->key, s)==0) {
+      p->count++;
+      return;
+    }
+  }
+}  
+
+void incr (struct hashtable *table, char *s) {
+  unsigned int h = hash(s);
+  unsigned int b = h % N;
+  incr_list (& table->buckets[b], s);
+}
+*)
+
+(* ================================================================= *)
+(** ** A functional model *)
+
+(** Before we prove the C program correct, we write a functional
+ program that models its behavior as closely as possible.  
+ The functional program won't be (average) constant time per access,
+ like the C program, because it takes linear time to get the nth
+ element of a list, while the C program can subscript an array in
+ constant time.  But we are not worried about the execution time
+ of the functional program; only that it serve as a model
+ for specifying the C program. *)
+
+
+Require Import VST.floyd.functional_base.
+Require ReflOmegaCore.
+
+Definition string := list byte.
+Instance EqDec_string: EqDec string := list_eq_dec Byte.eq_dec. 
+
+Fixpoint hashfun_aux (h: Z) (s: string) : Z :=
+ match s with
+ | nil => h
+ | c :: s' =>
+      hashfun_aux ((h * 65599 + Byte.signed c) mod Int.modulus) s'
+end.
+
+Definition hashfun (s: string) := hashfun_aux 0 s.
+
+Definition hashtable_contents := list (list (string * Z)).
+
+Definition N := 109.
+Lemma N_eq : N = 109. 
+Proof. reflexivity. Qed.
+Hint Rewrite N_eq : rep_omega.
+Global Opaque N.
+
+Definition empty_table : hashtable_contents :=
+  list_repeat (Z.to_nat N) nil.
+
+Fixpoint list_get (s: string) (al: list (string * Z)) : Z :=
+  match al with
+ | (k,i) :: al' => if eq_dec s k then i else list_get s al'
+ | nil => 0
+ end.
+
+Fixpoint list_incr (s: string) (al: list (string * Z))
+              :  list (string * Z) :=
+  match al with
+ | (k,i) :: al' => if eq_dec s k 
+                      then (k, i +1)::al'
+                      else (k,i)::list_incr s al'
+ | nil => (s, 1)::nil
+ end.
+
+Definition hashtable_get  (s: string) (contents: hashtable_contents) : Z :=
+  list_get s (Znth (hashfun s mod (Zlength contents)) contents).
+
+Definition hashtable_incr (s: string) (contents: hashtable_contents)
+                      : hashtable_contents :=
+  let h := hashfun s mod (Zlength contents)
+  in let al := Znth h contents
+  in upd_Znth h contents (list_incr s al).
+
+(** **** Exercise: 2 stars (hashfun_inrange)  *)
+
+Lemma mod_range: forall z m: Z, 0 < m -> 0 <= z mod m <= m - 1.
+Proof.
+  intros.
+  assert(0 <= z mod m < m). {
+    apply Z.mod_pos_bound; auto.
+  }
+  omega.
+Qed.
+
+Lemma mod_in_range: forall z : Z, 0 <= (z mod Int.modulus) <= Int.max_unsigned.
+Proof.
+  intros.
+  unfold Int.max_unsigned.
+  assert(4294967296 = Int.modulus). {
+    compute; reflexivity.
+  }
+  rewrite <- H; clear H.
+  apply mod_range; omega.
+Qed.
+
+Lemma hashfun_aux_inrange: forall s h, 0 <= h <= Int.max_unsigned ->
+                                  0 <= hashfun_aux h s <= Int.max_unsigned.
+Proof.
+  induction s as [|h t].
+  - (* s is nil *)
+    intros.
+    auto.
+  - (* s is h :: t *)
+    intros.
+    simpl.
+    apply IHt.
+    apply mod_in_range.
+Qed.
+
+Lemma hashfun_inrange: forall s, 0 <= hashfun s <= Int.max_unsigned.
+Proof.
+  unfold hashfun.
+  intros.
+  apply hashfun_aux_inrange.
+  rep_omega.
+Qed.
+
+(** [] *)
+
+(** **** Exercise: 1 star (hashfun_get_unfold)  *)
+Lemma hashtable_get_unfold:
+ forall sigma (cts: list (list (string * Z) * val)),
+ hashtable_get sigma (map fst cts) =
+  list_get sigma (Znth (hashfun sigma mod (Zlength cts)) (map fst cts)).
+Proof.
+  intros.
+  unfold hashtable_get.
+  rewrite Zlength_map.
+  auto.
+Qed.
+
+(** [] *)
+
+(** **** Exercise: 2 stars (Zlength_hashtable_incr)  *)
+Lemma Zlength_hashtable_incr:
+ forall sigma cts, 
+      0 < Zlength cts -> 
+      Zlength (hashtable_incr sigma cts) = Zlength cts.
+Proof.
+  intros.
+  unfold hashtable_incr.
+  rewrite upd_Znth_Zlength; auto.
+  apply Z.mod_pos_bound; auto.
+Qed.
+Hint Rewrite Zlength_hashtable_incr using list_solve : sublist.
+(** [] *)
+
+Lemma int_rep_helper: forall x y,
+    x mod Int.modulus = y  mod Int.modulus ->
+    Int.repr x = Int.repr y.
+Proof.
+  intros.
+  apply Int.eqm_samerepr.
+  unfold Int.eqm.
+  assert(0 < Int.modulus). {
+    rep_omega.
+  }
+  remember Int.modulus as b.
+  clear Heqb.
+  unfold Int.eqmod.
+  assert(x = b * (x / b) + (x mod b)). {
+    apply Z.div_mod.
+    rep_omega.
+  }
+  assert(y = b * (y / b) + (y mod b)). {
+    apply Z.div_mod.
+    rep_omega.
+  }
+  assert(y mod b = y - b * (y / b)). {
+    omega.
+  }
+  rewrite H in H1.
+  rewrite H3 in H1.
+  clear H H2 H3.
+  remember (x / b) as xb.
+  remember (y / b) as yb.
+  clear H0 Heqxb Heqyb.
+  exists (xb - yb).
+  rewrite Z.mul_comm.
+  rewrite H1; clear H1.
+  rewrite Z.mul_sub_distr_l.
+  rewrite Z.add_sub_assoc.
+  omega.
+Qed.
+
+Definition hash_step (hin: Z) (c: byte) :=
+  ((hin * 65599 + Byte.signed c) mod Int.modulus).
+
+Definition hashfun_aux' (h: Z) (s: string) :=
+  fold_left hash_step s h.
+
+Lemma hashfun_aux_equiv:
+  forall h s, hashfun_aux h s = hashfun_aux' h s.
+Proof.
+  intros.
+  revert h.
+  induction s as [| sh st].
+  - (* s is nil *)
+    intros.
+    unfold hashfun_aux.
+    unfold hashfun_aux'.
+    simpl.
+    auto.
+  - (* s is sh :: st *)
+    intros.
+    unfold hashfun_aux.
+    fold hashfun_aux.
+    rewrite IHst.
+    unfold hashfun_aux'.
+    unfold fold_left.
+    auto.
+Qed.
+
+Definition hash_step' (c: byte) (hin: Z) :=
+  hash_step hin c.
+
+Definition hashfun_aux'' (h: Z) (s: string) :=
+  fold_right hash_step' h (rev s).
+
+Lemma hashfun_aux_equiv':
+  forall h s, hashfun_aux' h s = hashfun_aux'' h s.
+Proof.
+  intros.
+  unfold hashfun_aux'.
+  unfold hashfun_aux''.
+  assert(hash_step = (fun x y => hash_step' y x)). {
+    unfold hash_step'.
+    unfold hash_step.
+    auto.
+  }
+  rewrite H.
+  rewrite fold_left_rev_right.
+  auto.
+Qed.
+
+Lemma hashfun_aux_equiv'':
+  forall h s, hashfun_aux h s = hashfun_aux'' h s.
+Proof.
+  intros.
+  rewrite hashfun_aux_equiv.
+  rewrite hashfun_aux_equiv'.
+  auto.
+Qed.
+
+Search (rev _ ++ rev _).
+Lemma hashfun_snoc0:
+  forall (s1 s2: string) (h: Z),
+    Int.repr (hashfun_aux h (s1 ++ s2)) =
+    Int.repr (hashfun_aux (hashfun_aux h s1) s2).
+Proof.
+  intros.
+  apply int_rep_helper.
+  rewrite hashfun_aux_equiv''.
+  rewrite hashfun_aux_equiv''.
+  rewrite hashfun_aux_equiv''.
+  unfold hashfun_aux''.
+  rewrite rev_app_distr.
+  rewrite fold_right_app.
+  auto.
+Qed.
+
+Lemma hashfun_snoc:
+  forall sigma h lo i,
+    0 <= lo ->
+    lo <= i < Zlength sigma ->
+  Int.repr (hashfun_aux h (sublist lo (i + 1) sigma)) =
+  Int.repr (hashfun_aux h (sublist lo i sigma) * 65599 + Byte.signed (Znth i sigma)).
+Proof.
+  intros.
+  assert(sublist lo (i + 1) sigma =
+         sublist lo i sigma ++ sublist i (i + 1) sigma). {
+    rewrite (sublist_split lo i (i+1)); try omega; auto.
+  }
+  rewrite H1. clear H1.
+  rewrite hashfun_snoc0.
+  rewrite sublist_len_1; try omega; auto.
+  apply int_rep_helper.
+  unfold hashfun_aux at 1.
+  rewrite Zmod_mod.
+  auto.
+Qed.
+
+(** [] *)
+
+(* ================================================================= *)
+(** ** Functional model satisfies the high-level specification *)
+
+(** The purpose of a hash table is to implement a finite mapping,
+  (a finite function) from keys to values.  We claim that the
+  functional model ([empty_table, hashtable_get, hashtable_incr])
+  correctly implements the appropriate operations on the abstract
+  data type of finite functions.
+
+  We formalize that statement by defining a Module Type: *)
+
+Module Type COUNT_TABLE.
+ Parameter table: Type.
+ Parameter key : Type.
+ Parameter empty: table.
+ Parameter get: key -> table -> Z.
+ Parameter incr: key -> table -> table.
+ Axiom gempty: forall k,   (* get-empty *)
+       get k empty = 0.
+ Axiom gss: forall k t,      (* get-set-same *)
+      get k (incr k t) = 1+(get k t).
+ Axiom gso: forall j k t,    (* get-set-other *)
+      j <> k -> get j (incr k t) = get j t.
+End COUNT_TABLE.
+
+(** This means:  in any [Module] that satisfies this [Module Type],
+   there's a type [table] of count-tables,
+   and operators [empty], [get], [set] that satisfy the axioms
+   [gempty], [gss], and [gso]. *)
+  
+(* ----------------------------------------------------------------- *)
+(** *** A "reference" implementation of COUNT_TABLE *)
+
+(** **** Exercise: 2 stars (FunTable)  *)
+(**  It's easy to make a slow implementation of [COUNT_TABLE], using functions. *)
+
+Module FunTable <: COUNT_TABLE.
+ Definition table: Type := nat -> Z.
+ Definition key : Type := nat.
+ Definition empty: table := fun k => 0.
+ Definition get (k: key) (t: table) : Z := t k.
+ Definition incr (k: key) (t: table) : table :=
+    fun k' => if Nat.eqb k' k then 1 + t k' else t k'.
+ Lemma gempty: forall k,  get k empty = 0.
+ Proof.
+   intros.
+   unfold get.
+   unfold empty.
+   auto.
+ Qed.
+ 
+ Lemma gss: forall k t,  get k (incr k t) = 1+(get k t).
+ Proof.
+   intros.
+   unfold get.
+   unfold incr.
+   rewrite Nat.eqb_refl.
+   auto.
+ Qed.
+ 
+ Lemma gso: forall j k t,  j <> k -> get j (incr k t) = get j t.
+ Proof.
+   intros.
+   unfold get.
+   unfold incr.
+   rewrite <- Nat.eqb_neq in H.
+   rewrite H.
+   auto.
+ Qed.
+ 
+End FunTable.
+(** [] *)
+
+(* ----------------------------------------------------------------- *)
+(** *** Demonstration that hash tables implement COUNT_TABLE *)
+
+(** **** Exercise: 3 stars (IntHashTable)  *)
+(**  Now we make a "fast" implementation using hash tables.  We
+  put "fast" in quotes because, unlike the imperative implementation,
+ the purely functional implementation takes linear time, not constant time,
+ to select the the i'th bucket.  That is, [Znth i al] takes time proportional to [i].
+ But that is no problem, because we are not using [hashtable_get] and
+ [hashtable_incr] as our real implementation; they are serving as the 
+ _functional model_ of the fast implementation in C.  *)
+
+Module IntHashTable <: COUNT_TABLE.
+ Definition hashtable_invariant (cts: hashtable_contents) : Prop :=
+  Zlength cts = N /\
+  forall i, 0 <= i < N ->
+             list_norepet (map fst (Znth i cts))
+             /\ Forall (fun s => hashfun s mod N = i) (map fst (Znth i cts)).
+ Definition table := sig hashtable_invariant.
+ Definition key := string.
+
+ Lemma empty_invariant: hashtable_invariant empty_table.
+ Proof.
+   
+   unfold empty_table.
+   unfold hashtable_invariant;split.
+   { (* Length *)
+     rewrite  Zlength_correct.
+     rewrite length_list_repeat.
+     rewrite Z2Nat.id; auto.
+     rewrite N_eq.
+     omega.
+   }
+   
+   { intros;split.
+     { (* list_norepet (map fst (Znth i (list_repeat (Z.to_nat N) nil))) *)
+       rewrite Znth_list_repeat_inrange;auto.
+       simpl.
+       apply list_norepet_nil.
+     }
+     { (* Forall (fun s : string => hashfun s mod N = i)
+          (map fst (Znth i (list_repeat (Z.to_nat N) nil))) *)  
+       rewrite Znth_list_repeat_inrange;auto.
+       simpl.
+       constructor.
+     }
+   }
+ Qed.
+
+ Lemma list_incr_in_existing:
+   forall (s: string) (al: list (string * Z)),
+     (In s (map fst al)) ->
+     (map fst (list_incr s al)) = (map fst al).
+ Proof.
+   intros.
+   induction al as [|hd tl].
+   - (* al is nil *)
+     inversion H.
+   - (* al is hd :: tl *)
+     destruct hd as [hs hz].
+     simpl in *.
+     destruct (eq_dec s hs) eqn: dshs.
+     * simpl;auto.
+     * simpl.
+       f_equal.
+       apply IHtl.
+       destruct H; auto.
+       subst hs. contradiction.
+ Qed.
+ 
+ Lemma list_incr_not_in_existing:
+   forall (s: string) (al: list (string * Z)),
+     ~ (In s (map fst al)) ->
+     (map fst (list_incr s al)) = (map fst al) ++ s :: nil.
+ Proof.
+   intros.
+   revert H.
+   induction al as [|hd tl].
+   - (* al is nil *)
+     intros.
+     simpl; auto.
+   - (* al is hd :: tl *)
+     intros.
+     destruct hd as [hs hz].
+     simpl in *.
+     assert(hs <> s /\ ~ In s (map fst tl)). {
+        split.
+        - unfold not.
+          intro.
+          subst hs.
+          apply H.
+          left;auto.
+        - intro.
+          apply H.
+          right;auto.
+     }
+     destruct H0.
+     destruct (eq_dec s hs) eqn: dshs.
+     * subst hs.
+       contradiction.
+     * simpl in *.
+       f_equal.
+       apply IHtl;auto.
+ Qed.
+
+ Lemma list_incr_not_in:
+   forall (s hstring : string) (t : list (string * Z)),
+     ~ In hstring (map fst t) ->
+     s <> hstring -> ~ In hstring (map fst (list_incr s t)).
+ Proof.
+   intros s hstring t H2 n.
+   assert(forall l l' : list byte, {l = l'} + {l <> l'}). {
+     apply list_eq_dec.
+     apply Byte.eq_dec.
+   }
+   destruct (ListDec.In_dec H s (map fst t)) eqn: si.
+   - rewrite list_incr_in_existing; auto.
+   - rewrite list_incr_not_in_existing; auto.
+     intro.
+     remember (map fst t) as ts.
+     remember (s :: nil) as ssingle.
+     Search app.
+     apply in_app_or in H0.
+     destruct H0; try contradiction.
+     subst ssingle.
+     simpl in *.
+     destruct H0; try contradiction.
+ Qed.
+ 
+ Lemma list_incr_nodup:
+   forall (s: string) (al: list (string * Z)),
+     list_norepet (map fst al) -> list_norepet (map fst (list_incr s al)).
+ Proof.
+   intros.
+   induction al as [|h t].
+   - (* al is nil *)
+     vm_compute.
+     assert(~In s nil). {
+       auto.
+     }
+     apply (list_norepet_cons s H0).
+     constructor.
+   - inversion H.
+     simpl.
+     destruct h as [hstring hcount].
+     simpl in *.
+     destruct (eq_dec s hstring) eqn: sh.
+     * simpl.
+       apply list_norepet_cons; auto.
+     * simpl in *.
+       apply list_norepet_cons; auto.
+       apply list_incr_not_in; auto.
+ Qed.
+
+Check ReflOmegaCore.ZOmega.IP.beq_reflect.
+ Lemma incr_invariant:
+   forall k cts, hashtable_invariant cts -> hashtable_invariant (hashtable_incr k cts).
+ Proof.
+   intros.
+   destruct H.
+   unfold hashtable_incr.
+   split.
+   { (* Length unchanged *)
+     rewrite upd_Znth_Zlength; auto.
+     assert(forall (A: Type) (l: list A), 0 <= Zlength l). {
+       intros.
+       apply (Zlength_nonneg l).
+     }
+     specialize (H1 (list (string * Z)) cts).
+     rewrite H in *.
+     rewrite N_eq in *.
+     generalize (hashfun k).
+     intros.
+     apply Z.mod_pos_bound; omega.
+   }
+   intros.
+   split.
+   {
+     (* list_norepet *)
+     remember (hashfun k mod Zlength cts) as bucket.
+     destruct (ReflOmegaCore.ZOmega.IP.beq_reflect bucket i).
+     { (* bucket = i *)
+       subst i.
+       rewrite <- H in *.
+       rewrite upd_Znth_same; auto.
+       apply list_incr_nodup.
+       specialize (H0 bucket).
+       apply H0 in H1.
+       destruct H1; auto.
+     }
+     { (* bucket != i *)
+       rewrite <- H in *.
+       rewrite upd_Znth_diff; auto.
+       specialize (H0 i).
+       apply H0 in H1.
+       destruct H1;auto.
+       subst bucket.
+       rewrite H in *.
+       rewrite N_eq in *.
+       apply Z.mod_pos_bound.
+       omega.
+     }
+   }
+   { (* All the strings in the ith bucket hash to i. *)
+     remember (hashfun k mod Zlength cts) as bucket.
+     destruct (ReflOmegaCore.ZOmega.IP.beq_reflect bucket i).
+     { (* bucket = i *)
+       subst i.
+       rewrite <- H in *.
+       rewrite upd_Znth_same; auto.
+       assert(forall l l' : list byte, {l = l'} + {l <> l'}). {
+         apply list_eq_dec.
+         apply Byte.eq_dec.
+       }
+       destruct (ListDec.In_dec H2 k (map fst (Znth bucket cts))) eqn: si.
+       { (* k is in the bucket already. *)
+         rewrite list_incr_in_existing; auto.
+         specialize (H0 bucket).
+         apply H0 in H1.
+         destruct H1; auto.
+       }
+       { (* k is not in the bucket. *)
+         rewrite list_incr_not_in_existing; auto.
+         specialize (H0 bucket).
+         apply H0 in H1.
+         destruct H1; auto.
+         apply Forall_app.
+         split; auto.
+       }
+     }
+     { (* bucket != i *)
+       rewrite <- H in *.
+       rewrite upd_Znth_diff; auto.
+       specialize (H0 i).
+       apply H0 in H1.
+       destruct H1;auto.
+       subst bucket.
+       rewrite H in *.
+       rewrite N_eq in *.
+       apply Z.mod_pos_bound.
+       omega.
+     }
+   }
+ Qed.
+ 
+
+ Definition empty : table := exist _ _ empty_invariant.
+ Definition get : key -> table -> Z := fun k tbl => hashtable_get k (proj1_sig tbl).
+ Definition incr : key -> table -> table := 
+       fun k tbl => exist _ _ (incr_invariant k _ (proj2_sig tbl)).
+
+
+ Theorem gempty: forall k, get k empty = 0.
+ Proof.
+   intros.
+   unfold empty.
+   unfold empty_table.
+   unfold get.
+   simpl.
+   unfold hashtable_get.
+   rewrite  Zlength_correct.
+   rewrite length_list_repeat.
+   assert(0 < N). {
+     rewrite N_eq;omega.
+   }
+   rewrite Z2Nat.id by omega.
+   remember (hashfun k mod N) as bucket.
+   assert(0 <= bucket < N). {
+     subst bucket.
+     apply Z.mod_pos_bound. auto.
+   }
+   rewrite Znth_list_repeat_inrange by auto.
+   simpl; auto.
+ Qed.
+ 
+ Lemma get_incr_result:
+   forall (k : key) (bklist : list (string * Z)),
+     list_get k (list_incr k bklist) = 1 + list_get k bklist.
+ Proof.
+   intros k bklist.
+   induction bklist as [|hd tl].
+   - (* bklist is  nil *)
+     simpl.
+     rewrite pred_dec_true;auto.
+   - (* inductive case *)
+     simpl.
+     destruct hd as [hk hz].
+     destruct (eq_dec k hk).
+     * rewrite pred_dec_true; auto.
+       unfold list_get.
+       rewrite pred_dec_true; auto.
+       rewrite pred_dec_true; auto.
+       rewrite Z.add_comm.
+       reflexivity.
+     * rewrite pred_dec_false; auto.
+       unfold list_get.
+       rewrite pred_dec_false; auto.
+       rewrite pred_dec_false; auto.
+ Qed.
+
+ Lemma get_incr_diff_result:
+   forall (j k : key) (bklist : list (string * Z)),
+     j <> k -> 
+     list_get j (list_incr k bklist) = list_get j bklist.
+ Proof.
+   intros j k bklist H.
+   induction bklist as [|hd tl].
+   - (* bklist is  nil *)
+     simpl.
+     rewrite pred_dec_false;auto.
+   - (* inductive case *)
+     simpl.
+     destruct hd as [hk hz].
+     destruct (eq_dec j hk).
+     * (* j = hk *)
+       rewrite (pred_dec_true (eq_dec j hk)); auto.
+       rewrite pred_dec_false.
+       simpl.
+       rewrite pred_dec_true; auto.
+       intro.
+       subst j k.
+       contradiction.
+     * (* j <> hk *)
+       rewrite (pred_dec_false (eq_dec j hk)); auto.
+       destruct (eq_dec k hk).
+     { (* k = hk *)
+       rewrite pred_dec_true.
+       simpl.
+       rewrite pred_dec_false; auto.
+       assumption.
+     }
+     { (* k <> hk *)
+       rewrite pred_dec_false; auto.
+       simpl.
+       rewrite pred_dec_false; auto.
+     }
+ Qed.
+
+ Theorem gss: forall k t,  get k (incr k t) =  1 + (get k t).
+ Proof.
+   intros.
+   unfold incr.
+   unfold get.
+   unfold hashtable_get.
+   unfold hashtable_incr.
+   destruct t.
+   simpl.
+   destruct h.
+   rewrite H in *.
+   rewrite N_eq in *.
+   remember (hashfun k mod 109) as bk.
+   assert(forall z : Z,
+             1 + z =
+             (match z with
+             | 0%Z => 1%Z
+             | Z.pos y' => Z.pos match y' with
+                                | q~1 => (Pos.succ q)~0
+                                | q~0 => q~1
+                                | 1 => 2
+                                end
+             | Z.neg y' => Z.pos_sub 1 y'
+              end)%positive). {
+     reflexivity.
+   }
+   rewrite <- H1.
+   assert(0 <= bk < Zlength x). {
+     rewrite Heqbk.
+     rewrite H.
+     apply Z.mod_pos_bound; omega.
+   }
+   rewrite upd_Znth_Zlength;auto.
+   rewrite H.
+   rewrite <- Heqbk.
+   rewrite upd_Znth_same;auto.
+   Search list_incr.
+   remember (Znth bk x) as bklist.
+   rewrite H in *.
+   apply get_incr_result.
+ Qed.
+ 
+ Theorem gso: forall j k t,    (* get-set-other *)
+      j <> k -> get j (incr k t) = get j t.
+ Proof.
+   intros j k t Hne.
+   unfold incr.
+   unfold get.
+   unfold hashtable_get.
+   unfold hashtable_incr.
+   destruct t.
+   simpl.
+   destruct h.
+   rewrite H in *.
+   rewrite N_eq in *.
+   remember (hashfun k mod 109) as bk.
+   assert(0 <= bk < Zlength x). {
+     rewrite Heqbk.
+     rewrite H.
+     apply Z.mod_pos_bound; omega.
+   }
+   rewrite upd_Znth_Zlength;auto.
+   remember (hashfun j mod 109) as bj.
+   assert(0 <= bj < Zlength x). {
+     rewrite Heqbj.
+     rewrite H.
+     apply Z.mod_pos_bound; omega.
+   }
+   rewrite H.
+   rewrite <- Heqbj.
+   destruct (Z.eq_dec bj bk) eqn:eqbjbk.
+   { (* bj = bk *)
+     rewrite e.
+     rewrite upd_Znth_same.
+     apply get_incr_diff_result; auto.
+     assumption.
+   }
+   { (* bj <> bk *)
+     rewrite upd_Znth_diff; auto.
+   }
+ Qed.
+
+(** [] *)
+
+End IntHashTable.
