formal/hash/Verif_hash.v
@@ -1,0 +1,1984 @@
+(** * Verif_hash: Correctness proof of hash.c *)
+
+Require Import VST.floyd.proofauto.
+Require Import VST.floyd.library.
+Require Import  Hash.hash.
+Instance CompSpecs : compspecs. make_compspecs prog. Defined.
+Definition Vprog : varspecs.  mk_varspecs prog. Defined.
+
+Require Import VST.msl.wand_frame.
+Require Import VST.msl.iter_sepcon.
+Require Import VST.floyd.reassoc_seq.
+Require Import VST.floyd.field_at_wand.
+Require Import Hash.Hashfun.
+
+(* ================================================================= *)
+(** ** Function specifications *)
+(* ----------------------------------------------------------------- *)
+(** *** Imports from the C string library *)
+
+Require Import DigUty.strlib_specs.
+Definition strcmp_spec := strcmp_spec' _strcmp 1 2.
+Definition strcpy_spec := strcpy_spec' _strcpy 1 2.
+Definition strlen_spec := strlen_spec' _strlen 1.
+
+(* ----------------------------------------------------------------- *)
+(** ***  String functions:  copy, hash *)
+
+Definition copy_string_spec : ident * funspec :=
+ DECLARE _copy_string
+ WITH sh: share, s: val, sigma : string, gv: globals
+ PRE [ _s OF tptr tschar ]
+    PROP (readable_share sh; Zlength sigma < Int.max_signed)
+    LOCAL (temp _s s; gvars gv)
+    SEP (mem_mgr gv; cstring sh sigma s)
+ POST [ tptr tschar ]
+    EX p: val, PROP ( ) LOCAL (temp ret_temp p)
+               SEP (cstring sh sigma s; cstring Ews sigma p;
+                      mem_mgr gv;
+                      malloc_token Ews (tarray tschar (Zlength sigma + 1)) p).
+
+Definition hash_spec : ident * funspec :=
+  DECLARE _hash
+  WITH sh: share, s: val, contents : string
+  PRE [ _s OF (tptr tschar) ]
+          PROP  (readable_share sh; Zlength contents < Int.max_signed)
+          LOCAL (temp _s s)
+          SEP   (cstring sh contents s)
+  POST [ tuint ]
+        PROP ()
+	LOCAL(temp ret_temp  (Vint (Int.repr (hashfun contents))))
+        SEP (cstring sh contents s).
+
+(* ----------------------------------------------------------------- *)
+(** *** Data structures for hash table *)
+
+Definition tcell := Tstruct _cell noattr.
+Definition thashtable := Tstruct _hashtable noattr.
+
+Definition list_cell (key: string) (count: Z) (next: val) (p: val): mpred :=
+ EX kp: val, cstring Ews key kp * data_at Ews tcell (kp,(Vint (Int.repr count), next)) p
+             * malloc_token Ews tcell p
+             * malloc_token Ews (tarray tschar (Zlength key + 1)) kp.
+
+Definition list_cell_local_facts:
+  forall key count next p, list_cell key count next p |-- !! isptr p.
+Proof. intros. unfold list_cell. Intros kp. entailer!. Qed.
+Hint Resolve list_cell_local_facts: saturate_local.
+
+Definition list_cell_valid_pointer:
+  forall key count next p, list_cell key count next p |-- valid_pointer p.
+Proof. intros. unfold list_cell. Intros kp. entailer!. Qed.
+Hint Resolve list_cell_valid_pointer: valid_pointer.
+
+(** **** Exercise: 1 star (listcell_fold)  *)
+Lemma listcell_fold: forall key kp count p' p,
+    cstring Ews key kp * data_at Ews tcell (kp, (Vint (Int.repr count), p')) p
+    * malloc_token Ews tcell p
+    * malloc_token Ews (tarray tschar (Zlength key + 1)) kp
+         |-- list_cell key count p' p.
+Proof.
+  intros.
+  unfold list_cell.
+  Exists kp.
+  entailer!.
+Qed.
+
+(** [] *)
+
+Fixpoint listrep (sigma: list (string * Z)) (x: val) : mpred :=
+ match sigma with
+ | (s,c)::hs => EX y: val, list_cell s c y x * listrep hs y
+ | nil =>
+    !! (x = nullval) && emp
+ end.
+
+(** **** Exercise: 2 stars (listrep_hints)  *)
+Lemma listrep_local_prop: forall sigma p, listrep sigma p |--
+        !! (is_pointer_or_null p  /\ (p=nullval <-> sigma=nil)).
+Proof.
+  intro sigma.
+  induction sigma as [| [hkey hcount] tl].
+  { (* sigma is nil *)
+    simpl.
+    entailer!.
+    split; reflexivity.
+  }
+  { (* sigma is (hkey, hcount) :: tl *)
+    intro p'.
+    simpl.
+    entailer.
+    saturate_local.
+    entailer!.
+    split.
+    {
+      intro.
+      subst p'.
+      contradiction.
+    }
+    {
+      intro.
+      inversion H0.
+    }
+  }
+Qed.
+
+Hint Resolve listrep_local_prop : saturate_local.
+
+Lemma listrep_valid_pointer:
+  forall sigma p,
+   listrep sigma p |-- valid_pointer p.
+Proof.
+  intro sigma.
+  induction sigma as [| [hkey hcount] tl].
+  { (* sigma is nil *)
+    simpl.
+    entailer!.
+  }
+  { (* sigma is (hkey, hcount) :: tl *)
+    intro p'.
+    simpl.
+    entailer.
+  }
+Qed.
+
+Hint Resolve listrep_valid_pointer : valid_pointer.
+(** [] *)
+
+Lemma listrep_fold: forall key count p' p al,
+  list_cell key count p' p * listrep al p' |-- listrep ((key,count)::al) p.
+Proof. intros. simpl. Exists p'. cancel. Qed.
+
+Lemma listrep_fold_nil: forall key count (p: val),
+  list_cell key count nullval p |-- listrep ((key,count)::nil) p.
+Proof.
+  intros. simpl.
+  Exists nullval.
+  entailer!.
+Qed.
+
+Definition listboxrep al r :=
+ EX p:val, data_at Tsh (tptr tcell) p r * listrep al p.
+
+Definition uncurry {A B C} (f: A -> B -> C) (xy: A*B) : C :=
+  f (fst xy) (snd xy).
+
+Definition hashtable_rep (contents: hashtable_contents) (p: val) : mpred :=
+  EX bl: list (list (string * Z) * val),
+    !! (contents = map fst bl) &&
+    malloc_token Ews thashtable p *
+    field_at Ews thashtable [StructField _buckets] (map snd bl) p
+    * iter_sepcon (uncurry listrep) bl.
+
+
+(** **** Exercise: 2 stars (hashtable_rep_hints)  *)
+Lemma hashtable_rep_local_facts: forall contents p,
+ hashtable_rep contents p |-- !! (isptr p /\ Zlength contents = N).
+Proof.
+  intros.
+  unfold hashtable_rep.
+  entailer.
+  saturate_local.
+  hint.
+  autorewrite with sublist.
+  entailer!.
+  rewrite N_eq.
+  inversion H1.
+  simpl in *.
+  unfold unfold_reptype in H2.
+  simpl in H2.
+  rewrite Zlength_map in H2.
+  auto.
+Qed.
+
+Hint Resolve hashtable_rep_local_facts : saturate_local.
+
+Lemma hashtable_rep_valid_pointer: forall contents p,
+ hashtable_rep contents p |-- valid_pointer p.
+Proof.
+  intros.
+  unfold hashtable_rep.
+  entailer.
+Qed.
+
+
+Hint Resolve hashtable_rep_valid_pointer : valid_pointer.
+(** [] *)
+
+(* ----------------------------------------------------------------- *)
+(** *** Function specifications for hash table *)
+
+Definition new_table_spec : ident * funspec :=
+ DECLARE _new_table
+ WITH u: unit, gv: globals
+ PRE [ ]
+   PROP()
+   LOCAL(gvars gv)
+   SEP(mem_mgr gv)
+ POST [ tptr thashtable ]
+   EX p:val, PROP()
+      LOCAL(temp ret_temp p)
+      SEP(mem_mgr gv; hashtable_rep empty_table p).
+
+Definition new_cell_spec : ident * funspec :=
+ DECLARE _new_cell
+ WITH sh: share, s: val, key: string, count: Z, next: val, gv: globals
+ PRE [ _key OF tptr tschar, _count OF tint, _next OF tptr tcell ]
+   PROP(readable_share sh; Zlength key < Int.max_signed)
+   LOCAL(temp _key s; temp _count (Vint (Int.repr count)); temp _next next; gvars gv)
+   SEP(mem_mgr gv; cstring sh key s)
+ POST [ tptr tcell ]
+   EX p:val, PROP()
+      LOCAL(temp ret_temp p)
+      SEP(list_cell key count next p; cstring sh key s;
+          mem_mgr gv).
+
+Definition get_spec : ident * funspec :=
+ DECLARE _get
+ WITH sh: share, p: val, contents: hashtable_contents, s: val, sigma : string
+ PRE [ _table OF tptr thashtable, _s OF tptr tschar ]
+    PROP (readable_share sh; Zlength sigma < Int.max_signed)
+    LOCAL (temp _table p; temp _s s)
+    SEP (hashtable_rep contents p; cstring sh sigma s)
+ POST [ tuint ]
+      PROP ( ) LOCAL (temp ret_temp (Vint (Int.repr (hashtable_get sigma contents))))
+      SEP (hashtable_rep contents p; cstring sh sigma s).
+
+Definition incr_list_spec : ident * funspec :=
+ DECLARE _incr_list
+ WITH sh: share, r0: val, al: list (string * Z), s: val, sigma : string
+ PRE [ _r0 OF tptr (tptr tcell), _s OF tptr tschar ]
+    PROP (readable_share sh; Zlength sigma < Int.max_signed; list_get sigma al < Int.max_unsigned)
+    LOCAL (temp _r0 r0; temp _s s)
+    SEP (listboxrep al r0; cstring sh sigma s)
+ POST [ tvoid ]
+      PROP ( ) LOCAL ()
+      SEP (listboxrep (list_incr sigma al) r0; cstring sh sigma s).
+
+Definition incr_spec : ident * funspec :=
+ DECLARE _incr
+ WITH sh: share, p: val, contents: hashtable_contents, s: val, sigma : string
+ PRE [ _table OF tptr thashtable, _s OF tptr tschar ]
+    PROP (readable_share sh; Zlength sigma < Int.max_signed; 
+          hashtable_get sigma contents < Int.max_unsigned)
+    LOCAL (temp _table p; temp _s s)
+    SEP (hashtable_rep contents p; cstring sh sigma s)
+ POST [ tvoid ]
+      PROP ( ) LOCAL ()
+      SEP (hashtable_rep (hashtable_incr sigma  contents) p; cstring sh sigma s).
+
+(**  Putting all the funspecs together *)
+
+Definition Gprog : funspecs :=
+        ltac:(with_library prog [
+                   strcmp_spec; strcpy_spec; strlen_spec; hash_spec;
+                   new_cell_spec; copy_string_spec; get_spec; incr_spec;
+                   incr_list_spec
+ ]).
+
+(* ================================================================= *)
+(** ** Proofs of the function bodies *)
+
+(** This lemma demonstrates how to handle "strings", that is,
+   null-terminated arrays of characters. *)
+Lemma demonstrate_cstring1:
+ forall i contents,
+   ~ In Byte.zero contents ->
+   Znth i (contents ++ [Byte.zero]) <> Byte.zero  ->
+   0 <= i <= Zlength contents ->
+   0 <= i + 1 < Zlength (contents ++ [Byte.zero]).
+Proof.
+intros.
+(** When processing a C null-terminated string, you will want to
+   maintain the three kinds of assumptions above the line.
+   A string is an array of characters with three parts:
+   - The "contents" of the string, none of which is the '\0' character;
+   - The null termination character, equal to Byte.zero;
+   - the remaining garbage in the array, after the null.
+  The first assumption above the line says that none of the
+  contents is the null character.
+  Now suppose we are in a loop where variable [_i] (with value [i])
+  is traversing the array.  We expect that loop to go up to but
+  no farther than the null character, that is, one past the contents.
+  Therefore [0 <= i <= Zlength contents].
+  Furthermore, suppose we have determined (by an if-test) that
+  s[i] is not zero, then we have the hypothesis H0 above.
+
+  The [cstring] tactic processes all three of them to conclude
+  that [i < Zlength contents]. *)
+assert (H7: i < Zlength contents) by cstring.
+
+(** But actually, [cstring] tactic will prove any rep_omega consequence
+   of that fact.  For example: *)
+clear H7.
+autorewrite with sublist.
+cstring.
+Qed.
+(** Don't apply [demonstrate_cstring1] in the body_hash proof,
+    instead, use [autorewrite with sublist] and [cstring] directly,
+    where appropriate. *)
+
+Lemma demonstrate_cstring2:
+ forall i contents,
+   ~ In Byte.zero contents ->
+   Znth i (contents ++ [Byte.zero]) = Byte.zero  ->
+   0 <= i <= Zlength contents ->
+   i = Zlength contents.
+Proof.
+intros.
+(** Here is another demonstration.  When your loop on the
+   string contents reaches the end, so that s[i] is the zero byte,
+   you'll have the an assumption like [H0] above the line.
+   The [cstring] tactic handles this case too, to prove
+   [i = Zlength contents].   *)
+cstring.
+Qed.
+
+(** **** Exercise: 3 stars (body_hash)  *)
+Lemma body_hash: semax_body Vprog Gprog f_hash hash_spec.
+Proof.
+start_function.
+unfold cstring,hashfun in *.
+(** Before doing this proof, study some of the proofs in VST/progs/verif_strlib.v.
+  In the PROP part of your loop invariant, you'll want to maintain [0 <= i <= Zlength contents].
+
+  In the LOCAL part of your loop invariant, try to use something like
+
+    temp _c (Vbyte (Znth i (contents ++ [Byte.zero]))
+
+  instead of
+
+    temp _c (Znth 0 (map Vbyte (...)))
+
+  The reason is that [temp _c (Vint x)] or [temp _c (Vbyte y)] is much easier
+  for Floyd to handle than [temp _c X]
+  where X is a general formula of type [val].
+
+  Late in the proof of the loop body, the lemma [hashfun_snoc] will be useful. *)
+forward.
+forward.
+forward.
+entailer!.
+forward_while
+  (EX i:Z,
+    PROP (0 <= i < (Zlength contents + 1))
+    LOCAL (temp _c (Vbyte (Znth i (contents ++ [Byte.zero])));
+           temp _i (Vint (Int.repr i));
+           temp _n (Vint (Int.repr (hashfun_aux 0 (sublist 0 i contents))));
+           temp _s s)
+    SEP (!! (~ In Byte.zero contents) &&
+                 data_at sh (tarray tschar (Zlength contents + 1)) (map Vbyte (contents ++ [Byte.zero])) s)).
+{ (* Current pre implies invariant. *)
+  Exists 0.
+  entailer!.
+}
+{ (* Type Check *)
+  entailer!.
+}
+{ (* Now in the loop body. *)
+  forward.
+  forward.
+  assert(i <> Zlength contents). {
+    intro.
+    subst i.
+    simpl in HRE.
+    rewrite app_Znth2 in HRE.
+    rewrite Z.sub_diag in HRE.
+    unfold Znth in HRE.
+    simpl in HRE.
+    contradiction.
+    (* Now must prove Zlength contents >= Zlength contents *)
+    omega.
+  }
+  assert(0 <= i < Zlength contents). {
+    omega.
+  }
+  forward.
+  Exists (i + 1).
+  entailer!.
+  f_equal.
+  rewrite app_Znth1 by omega.
+  apply (hashfun_snoc contents 0 0 i);omega.
+}
+{ (* At the return *)
+  forward.
+  entailer!.
+  f_equal.
+  assert(i = Zlength contents). {
+    assert(~ (0 <= i < Zlength contents)). {
+      intro.
+      rewrite app_Znth1 in HRE by omega.
+      assert(In (Znth i contents) contents). {
+        apply Znth_In; auto.
+      }
+      rewrite HRE in H6.
+      contradiction.
+    }
+    omega.
+  }
+  subst i.
+  rewrite sublist_same by omega.
+  reflexivity.
+}
+Qed.
+
+(** [] *)
+
+(** **** Exercise: 3 stars (body_new_cell)  *)
+
+Lemma body_copy_string: semax_body Vprog Gprog f_copy_string copy_string_spec.
+Proof.
+  start_function.
+  forward_call (sh, sigma, s). (* strlen *)
+  forward.
+  forward_call ((tarray tschar (Zlength sigma + 1)), gv). (* to malloc *)
+  {
+    (* Prove Zlength size + 1 in two forms are equal. *)
+    entailer!.
+    repeat f_equal.
+    assert(Int.signed (Int.repr 1) = 1). {
+      (* Search (Int.signed (Int.repr _)).*)
+      apply Int.signed_repr.
+      rep_omega.
+    }
+    rewrite H1.
+    (* Search (Int64.unsigned (Int64.repr _)). *)
+    assert((Int64.unsigned (Int64.repr (Zlength sigma + 1))) = (Zlength sigma + 1)). {
+      apply Int64.unsigned_repr.
+      rep_omega.
+    }
+    rewrite H2.
+    Search (Int.signed (Int.repr _)).
+    apply Int.signed_repr.
+    rep_omega.
+  }
+  {
+    split3; simpl; auto.
+    rewrite Z.max_r; rep_omega.
+  }
+  {
+    Intros p.
+    forward_if
+      (PROP ( )
+       LOCAL (temp _p p; temp _s s;gvars gv)
+       SEP (mem_mgr gv;
+            malloc_token Ews (tarray tschar (Zlength sigma + 1)) p;
+            cstring sh sigma s;
+            data_at_ Ews (tarray tschar (Zlength sigma + 1)) p)).
+    {
+      change (Memory.EqDec_val p nullval) with (eq_dec p nullval).
+      if_tac; entailer!.
+    }
+    {
+      forward_call tt. (* Call to exit *)
+      contradiction.
+    }
+    {
+      rewrite if_false by auto.
+      Intros.
+      forward.  (*  /*skip*/;  *)
+      entailer.
+      unfold cstring.
+      entailer!.
+    }
+    (* Call to strcpy *)
+    forward_call (Ews, sh, p, (Zlength sigma + 1), s, sigma).
+    split3; auto.
+    omega.
+    forward.
+    Exists p.
+    entailer!.
+    unfold cstringn, cstring.
+    entailer!.
+    assert((Zlength sigma + 1 - (Zlength sigma + 1)) = 0). {
+      rep_omega.
+    }
+    rewrite H7.
+    assert(Z.to_nat 0 = 0%nat). {
+      reflexivity.
+    }
+    rewrite H8.
+    simpl.
+    entailer!.
+    rewrite app_nil_r.
+    entailer!.
+  }
+Qed.
+
+Lemma body_new_cell: semax_body Vprog Gprog f_new_cell new_cell_spec.
+Proof.
+  start_function.
+  forward_call (tcell, gv). (* malloc *)
+  {
+    (* preconditions of malloc *)
+    split3; simpl; try rep_omega;auto.
+  }
+  Intros p.
+  forward_if
+    (PROP ( )
+     LOCAL (temp _p p; temp _key s; temp _count (Vint (Int.repr count)); temp _next next; gvars gv)
+     SEP (mem_mgr gv;
+          malloc_token Ews tcell p;
+          data_at_ Ews tcell p;
+          cstring sh key s)).
+  { (* *)
+    destruct  (Memory.EqDec_val p nullval);
+    if_tac;entailer!.
+  }
+  {
+    forward_call tt.
+    inversion H1.
+  }
+  {
+    rewrite if_false by auto.
+    forward.
+    entailer!.
+  }
+  { (* Call copy_string *)
+    forward_call (sh, s, key, gv).
+    Intros key_copy.
+    forward.
+    forward.
+    forward.
+    forward.
+    Exists p.
+    unfold list_cell.
+    Exists key_copy.
+    entailer!.
+  }
+
+Qed.
+
+(** [] *)
+
+(* ================================================================= *)
+(** ** Auxiliary lemmas about data-structure predicates *)
+
+
+(** **** Exercise: 2 stars (iter_sepcon_hints)  *)
+Lemma iter_sepcon_listrep_local_facts:
+ forall bl, iter_sepcon (uncurry listrep) bl
+                    |-- !! Forall is_pointer_or_null (map snd bl).
+Proof.
+(* Hint: use [induction] and [sep_apply]. *)
+  intros.
+  induction bl as [| h t].
+  { (* bl is nil *)
+    simpl.
+    entailer!.
+  }
+  { (* bl is h :: t *)
+    destruct h as [hc hp].
+    simpl.
+    sep_apply IHt.
+    unfold uncurry at 2.
+    simpl.
+    entailer!.
+  }
+Qed.
+
+
+Hint Resolve iter_sepcon_listrep_local_facts : saturate_local.
+(** [] *)
+
+(** **** Exercise: 2 stars (iter_sepcon_split3)  *)
+Lemma iter_sepcon_split3:
+  forall {A}{d: Inhabitant A} (i: Z) (al: list A) (f: A -> mpred),
+   0 <= i < Zlength al   ->
+  iter_sepcon f al =
+  iter_sepcon f (sublist 0 i al) * f (Znth i al) * iter_sepcon f (sublist (i+1) (Zlength al) al).
+Proof.
+intros.
+rewrite <- (sublist_same 0 (Zlength al) al) at 1 by auto.
+(* Hint: [rewrite (sublist_split LO MID HI) by omega], where you choose values for LO MID HI.
+  Also useful:  [rewrite sublist_len_1]    and    [iter_sepcon_app].
+*)
+rewrite (sublist_split 0 i (Zlength al)) by omega.
+rewrite (sublist_split i (i+1) (Zlength al)) by omega.
+rewrite (sublist_len_1 i); auto.
+rewrite iter_sepcon_app.
+rewrite iter_sepcon_app.
+simpl.
+remember (iter_sepcon f (sublist 0 i al)) as P1.
+remember (iter_sepcon f (sublist (i + 1) (Zlength al) al)) as P3.
+rewrite sepcon_emp.
+rewrite sepcon_assoc.
+reflexivity.
+Qed.
+
+(** [] *)
+
+(** **** Exercise: 3 stars (body_new_table)  *)
+Lemma body_new_table_helper:
+ (* This lemma is useful as the very last thing to do in body_new_table *)
+ forall p,
+   data_at
+     Ews thashtable (list_repeat (Z.to_nat N) nullval) p
+  |-- field_at Ews thashtable [StructField _buckets]
+       (list_repeat (Z.to_nat N) nullval) p *
+         iter_sepcon (uncurry listrep) (list_repeat (Z.to_nat N) ([], nullval)).
+Proof.
+intros.
+unfold_data_at 1%nat.
+entailer!.
+assert(forall n: nat, iter_sepcon (uncurry listrep) (list_repeat n ([], nullval)) = emp). {
+  intro n.
+  induction n as [|n'].
+  { (* n is 0 *)
+    simpl; auto.
+  }
+  { (* n is S n' *)
+    assert((forall nn: nat, S nn = 1 + nn)%nat). {
+      intros;reflexivity.
+    }
+    rewrite H1.
+    rewrite <- list_repeat_app.
+    simpl.
+    rewrite IHn'.
+    rewrite sepcon_emp.
+    unfold uncurry.
+    simpl.
+    autorewrite with norm.
+    auto.
+  }
+}
+rewrite (H1 (Z.to_nat N)).
+entailer.
+Qed.
+
+Lemma upd_single_repeat:
+  forall (A: Type) (old new: A),
+    upd_Znth 0 (list_repeat (Z.to_nat 1) old) new =
+    (list_repeat (Z.to_nat 1) new).
+Proof.
+  intros.
+  simpl.
+  unfold upd_Znth.
+  simpl.
+  unfold Zlength.
+  simpl.
+  rewrite sublist_nil.
+  reflexivity.
+Qed.
+
+
+Lemma body_new_table: semax_body Vprog Gprog f_new_table new_table_spec.
+Proof.
+(** The loop invariant in this function describes a partially initialized array.
+   The best way to do that is with something like,
+
+  data_at Tsh thashtable
+      (list_repeat (Z.to_nat i) nullval ++
+       list_repeat (Z.to_nat (N-i)) Vundef)   p.
+
+  Then at some point you'll have to prove something about,
+
+   data_at Tsh thashtable
+      (list_repeat (Z.to_nat (i + 1)) nullval ++
+       list_repeat (Z.to_nat (N - (i + 1))) Vundef)   p
+
+  In particular, you'll have to split up [list_repeat (Z.to_nat (i + 1)) nullval]
+   into [list_repeat (Z.to_nat i) nullval ++ list_repeat (Z.to_nat 1) nullval].
+  The best way to do that is [rewrite <- list_repeat_app'.]
+*)
+  start_function.
+  forward_call (thashtable, gv).
+  { (* preconditions of malloc *)
+    split3; simpl; try rep_omega;auto.
+  }
+  Intros p.
+  forward_if
+    (PROP (p <> nullval)
+     LOCAL (temp _p p; gvars gv)
+     SEP (mem_mgr gv;
+          malloc_token Ews thashtable p;
+          data_at_ Ews thashtable p)).
+  { (* *)
+    destruct  (Memory.EqDec_val p nullval).
+    * entailer!.
+    * rewrite if_false by auto.
+      entailer!.
+  }
+  {
+    forward_call tt.
+    inversion H0.
+  }
+  forward.
+  entailer!.
+  rewrite if_false by auto.
+  entailer!.
+  forward_for_simple_bound
+    109
+    (EX i:Z,
+          (PROP (p <> nullval)
+           LOCAL (temp _p p; gvars gv)
+           SEP (mem_mgr gv; malloc_token Ews thashtable p *
+                data_at Ews thashtable
+                        (list_repeat (Z.to_nat i) nullval ++
+                                     list_repeat (Z.to_nat (N-i)) Vundef)
+                        p)))%assert.
+  { (* Proof pre-state implies the invariant *)
+    entailer!.
+    simpl.
+    unfold data_at_, data_at, field_at_.
+    entailer!.
+  }
+  {
+    Intros.
+    forward.
+    rewrite Z2Nat.inj_add by omega.
+    rewrite <- list_repeat_app.
+    assert((N-i) = 1 + (N - (i+1))). {
+      omega.
+    }
+    rewrite H1.
+    rewrite Z2Nat.inj_add; try omega.
+    rewrite <- list_repeat_app.
+    rewrite upd_Znth_app2.
+    {
+      rewrite Zlength_list_repeat by omega.
+      assert(i - i = 0). {
+        omega.
+      }
+      rewrite H2.
+      rewrite upd_Znth_app1.
+      {
+        remember (list_repeat (Z.to_nat i) nullval) as part1.
+        remember (list_repeat (Z.to_nat (N - (i + 1))) Vundef) as part3.
+        rewrite upd_single_repeat.
+        assert(Int.unsigned (Int.repr 0) = 0). {
+          rewrite Int.unsigned_repr; [reflexivity | rep_omega].
+        }
+        rewrite H3.
+        entailer!.
+        assert(Vlong (Int64.repr 0) = nullval). {
+          unfold nullval.
+          unfold Archi.ptr64.
+          reflexivity.
+        }
+        rewrite H7.
+        rewrite app_assoc.
+        entailer!.
+      }
+      {
+        rewrite Zlength_list_repeat; omega.
+      }
+    }
+    {
+      rewrite Zlength_list_repeat by omega.
+      rewrite Zlength_app.
+      rewrite Zlength_list_repeat by omega.
+      rewrite Zlength_list_repeat.
+      {
+        rewrite <- H1.
+        rewrite N_eq in *.
+        omega.
+      }
+      {
+        rewrite N_eq in *.
+        omega.
+      }
+    }
+    rewrite N_eq in *.
+    omega.
+  }
+  { (* At return. *)
+    forward.
+    rewrite <- N_eq in *.
+    rewrite Z.sub_diag in *.
+    simpl in *.
+    rewrite <- app_nil_end in *.
+    Exists p.
+    entailer!.
+    unfold hashtable_rep.
+    Exists (list_repeat (Z.to_nat N) ((@nil (string * Z)), nullval)).
+    entailer!.
+    assert((map snd (list_repeat (Z.to_nat N) ((@nil (string * Z), nullval)))) =
+           (list_repeat (Z.to_nat N) nullval)). {
+      rewrite map_list_repeat.
+      reflexivity.
+    }
+    rewrite H4.
+    apply (body_new_table_helper p).
+  }
+
+Qed.
+
+(** [] *)
+
+(** **** Exercise: 3 stars (body_get)  *)
+(** The [get] function traverses a linked list.  We will reason about linked-list traversal
+   in separation logic using "Magic Wand as Frame" http://www.cs.princeton.edu/~appel/papers/wand-frame.pdf
+   When the loop is partway down the linked list, we can view the original list
+   up to the current position as a "linked-list data structure with a hole";
+   and the current position points to a linked-list data structure that fills the hole.
+   The "data-structure-with-a-hole" we reason about with separating implication,
+    called "magic wand":   (hole -* data-structure)
+    which says, if you can conjoin this data-structure-with-a-hole
+    with something-to-fill-the-hole, then you get the original data structure:
+     hole * (hole -* data-structure) |--   data-structure.
+    The lemma [listrep_traverse] is useful in moving one linked-list cell
+    out of the hole and into the data-structure-with-a-(smaller)-hole.
+*)
+
+Lemma listrep_traverse:  (* useful in body_get lemma*)
+  forall key count p' p,
+  list_cell key count p' p |--
+  ALL al:list (string * Z), listrep al p' -* (EX y : val, list_cell key count y p * listrep al y).
+Proof.
+intros.
+apply allp_right. intro al.
+apply wand_sepcon_adjoint.
+Exists p'.
+entailer!.
+Qed.
+
+Lemma is_pointer_or_null_expand:
+  forall p: val, is_pointer_or_null p -> isptr p \/ p = nullval.
+Proof.
+  intros.
+  destruct p;simpl in *; try inversion H.
+  { (* Vlong *)
+    right; auto.
+  }
+  { (* Vptr *)
+    left;auto.
+  }
+Qed.
+
+Lemma isptr_expand:
+  forall p: val, isptr p -> exists (b : block) (o: ptrofs), p = Vptr b o.
+Proof.
+  intros.
+  destruct p eqn: ?; try (simpl in H; inversion H).
+  exists b.
+  exists i.
+  reflexivity.
+Qed.
+
+Lemma wand_cancel:
+  forall P Q R,
+    P * (P * Q -* R) |-- Q -* R.
+Proof.
+  intros.
+  rewrite <- wand_sepcon_adjoint.
+  rewrite sepcon_assoc.
+  rewrite (sepcon_comm (P * Q -* R) Q).
+  rewrite <- sepcon_assoc.
+  apply modus_ponens_wand.
+Qed.
+
+Lemma wand_cancel':
+  forall P Q R,
+    Q * P * (P * Q -* R) |-- Q * (Q -* R).
+Proof.
+  intros.
+  sep_apply (wand_cancel P Q R).
+  rewrite sepcon_comm.
+  auto.
+Qed.
+
+Lemma emp_wand:
+  forall P,
+    (emp -* P) = P.
+Proof.
+  intros.
+  apply pred_ext.
+  { (* emp -* P |-- P *)
+    rewrite <- (sepcon_emp (emp -* P)).
+    rewrite sepcon_comm.
+    apply modus_ponens_wand.
+  }
+  { (* P |-- emp -* P *)
+    apply wand_sepcon_adjoint.
+    rewrite sepcon_emp.
+    auto.
+  }
+Qed.
+
+Lemma exp_eq:
+  forall (A: Type) (P: A -> mpred),
+    (EX y: A, P y) = (EX y':A, P y').
+Proof.
+  auto.
+Qed.
+
+Lemma sepcon_exp:
+  forall (A: Type) (y: A) (P Q: A -> mpred),
+    (P y) * (Q y) |--  (EX y':A, (P y') * (Q y')).
+Proof.
+  intros.
+  apply (exp_right y).
+  auto.
+Qed.
+
+Lemma sepcon_exp':
+  forall (A: Type) (y: A) (P: A -> mpred),
+    (P y) |--  (EX y':A, (P y')).
+Proof.
+  intros.
+  apply (exp_right y).
+  auto.
+Qed.
+
+(*
+Lemma wand_ex_intro:
+  forall (A: Type) (y: A) (P: A -> mpred) (Q: mpred),
+    (EX y':A, (P y')) -* Q |--  ((P y) -* Q).
+Proof.
+  intros.
+  remember (EX y' : A, P y') as x'.
+  rewrite <- (wand_sepcon_adjoint
+Qed.
+*)
+Lemma wand_cancel_ex:
+  forall (A: Type) (y: A) (P Q: A -> mpred) (R: mpred),
+    (P y) * ((EX y':A, ((P y') * (Q y'))) -* R) |-- (Q y) -* R.
+Proof.
+  intros.
+  rewrite <- wand_sepcon_adjoint.
+  sep_apply (sepcon_exp A y P Q).
+  apply wand_frame_elim.
+Qed.
+
+Lemma wand_cancel_ex':
+  forall (A: Type) (y: A) (P Q: A -> mpred) (R: mpred),
+    (Q y) * (P y) * ((EX y':A, ((P y') * (Q y'))) -* R) |-- R.
+Proof.
+  intros.
+  rewrite sepcon_assoc.
+  rewrite sepcon_comm.
+  rewrite wand_sepcon_adjoint.
+  sep_apply (wand_cancel_ex A y P Q R).
+  auto.
+Qed.
+
+Lemma body_get: semax_body Vprog Gprog f_get get_spec.
+Proof.
+  start_function.
+  rename p into table.
+  pose proof (hashfun_inrange sigma).
+  forward_call (sh, s, sigma). (* h = hash(s) *)
+  forward.
+  rewrite modu_repr; [| auto |  rep_omega].
+  remember ((hashfun sigma) mod 109) as bk.
+  assert(0 <= bk < 109). {
+    rewrite Heqbk.
+    apply (Z.mod_pos_bound (hashfun sigma) 109); omega.
+  }
+  unfold hashtable_rep.
+  Intros bl.
+  remember (map snd bl) as buckets.
+  forward.
+  {
+    
+    entailer.
+  }
+  {
+    entailer!.
+    simplify_value_fits in H3.
+    destruct H3.
+    autorewrite with sublist in *|-.
+    remember ((hashfun sigma) mod 109) as bk.
+    assert(0 <= bk < Zlength bl). {
+      rewrite H0.
+      rewrite Heqbk.
+      apply (Z.mod_pos_bound (hashfun sigma) 109); omega.
+    }
+    rewrite Znth_map by auto.
+    rewrite Forall_map in H4.
+    apply Forall_Znth; auto.
+  }
+{
+  rewrite <- Heqbk.
+  autorewrite with norm.
+  deadvars!.
+  assert_PROP(Zlength bl = 109). {
+    entailer!.
+    simplify_value_fits in H4.
+    destruct H4.
+    autorewrite with sublist in *|-.
+    auto.
+  }
+  assert(0 <= bk < Zlength bl). {
+    rewrite H1.
+    rewrite Heqbk.
+    apply (Z.mod_pos_bound (hashfun sigma) 109); omega.
+  }
+  rewrite (iter_sepcon_split3 bk bl (uncurry listrep) H2).
+
+  unfold uncurry at 2.
+  remember (Znth bk buckets) as p0.
+  remember (Znth bk contents) as l0.
+  rewrite <- (Znth_map bk fst bl) by auto.
+  rewrite <- (Znth_map bk snd bl) by auto.
+  rewrite <- Heqbuckets.
+  rewrite <- H0.
+  rewrite H1.
+  (* So p0 is pointing to l0 the list we now traverse. *)
+  forward_while (EX p: val, EX l: list (string * Z),
+     PROP (l0 = (Znth bk contents);
+           p0 = (Znth bk buckets);
+           list_get sigma l = list_get sigma l0)
+     LOCAL (temp _p p;
+            temp _s s)
+     SEP (cstring Tsh sigma s;
+          malloc_token Tsh thashtable table;
+          field_at Tsh thashtable [StructField _buckets] (map snd bl) table;
+          iter_sepcon (uncurry listrep) (sublist 0 bk bl);
+          listrep l p;
+          listrep l p -* listrep l0 p0;
+          iter_sepcon (uncurry listrep) (sublist (bk + 1) (Zlength bl) bl)))%assert.
+  { (* subgoal 1 *)
+    Exists p0 l0.
+    entailer!.
+    simplify_value_fits in H5.
+    destruct H5.
+    remember (listrep (Znth (hashfun sigma mod 109) (map fst bl)) (Znth (hashfun sigma mod 109) (map snd bl))) as P.
+    cancel.
+    autorewrite with sublist in *|-.
+    rewrite H0.
+    remember (iter_sepcon (uncurry listrep) (sublist (hashfun sigma mod 109 + 1) 109 bl)) as Q.
+    cancel.
+    apply wand_refl_cancel_right.
+  }
+  { (* subgoal 2 *)
+    entailer!.
+  }
+  { (* subgoal 3 *)
+    destruct l as [| lh lt].
+    { (* l is nil *)
+      unfold listrep at 2.
+      normalize.
+    }
+    { (* l is lh :: lt *)
+      unfold listrep at 2.
+      fold listrep.
+      unfold list_cell.
+      destruct lh as [key count].
+      Intros y kp.
+      forward.
+      forward_call (kp, key, s, sigma).
+      Intros strcmp_ret.
+      forward_if.
+      { (* True branch *)
+        rewrite pred_dec_true in H6 by auto.
+        simpl in H5.
+        rewrite pred_dec_true in H5 by auto.
+        forward.
+        sep_apply (listcell_fold key kp count y p).
+        sep_apply (listrep_fold key count y p lt).
+        sep_apply (wand_frame_elim (listrep ((key, count) :: lt) p) (listrep l0 p0)).
+        assert((listrep l0 p0) = (uncurry listrep) (l0, p0)). {
+          unfold uncurry.
+          reflexivity.
+        }
+        rewrite H8.
+        assert((l0, p0) = Znth bk bl). {
+          subst l0 p0.
+          subst contents buckets.
+          rewrite Znth_map by auto.
+          rewrite Znth_map by auto.
+          remember (Znth bk bl) as bkbl.
+          rewrite <- surjective_pairing; reflexivity.
+        }
+        rewrite H9.
+        assert((iter_sepcon (uncurry listrep) (sublist 0 bk bl) *
+                uncurry listrep (Znth bk bl) *
+                iter_sepcon (uncurry listrep) (sublist (bk + 1) (Zlength bl) bl))
+                 |--
+                 (iter_sepcon (uncurry listrep) bl)). {
+          apply derives_refl''.
+          apply iter_sepcon_split3.
+          auto.
+        }
+        sep_apply H10.
+        forward.
+        entailer!.
+        {
+          unfold hashtable_get.
+          rewrite Zlength_map.
+          rewrite H1.
+          reflexivity.
+        }
+        {
+          unfold hashtable_rep.
+          Exists bl.
+          entailer!.
+        }
+      }
+      (* After the if. Apparently the empty else clause does have any requirements. *)
+      forward. (* Over p=p->next; *)
+
+      (* At end of loop. Show the invariant still holds. *)
+      rewrite if_false in H6 by auto.
+      Exists (y, lt).
+      simpl in H5.
+      rewrite if_false in H5.
+      2: auto.
+      sep_apply (listcell_fold key kp count y p).
+      simpl (listrep ((key, count) :: lt) p).
+      assert (list_cell key count y p *
+              ((EX y' : val, list_cell key count y' p * listrep lt y') -* listrep l0 p0)
+                |-- listrep lt y -* listrep l0 p0).
+      {
+        exact (wand_cancel_ex val y
+                                (fun y': val => list_cell key count y' p)
+                                (fun y': val => listrep lt y')
+                                (listrep l0 p0)).
+      }
+      sep_apply H8.
+      simpl (listrep (snd (y, lt)) (fst (y, lt))).
+      entailer!.
+    }
+  }
+  {
+    assert_PROP(l = nil). {
+      destruct l as [| [lhs lhx] lt].
+      { (* l is nil *)
+        entailer!.
+      }
+      { (* l id lh :: lt *)
+        unfold listrep at 2.
+        Intros y.
+        fold (listrep lt y).
+        assert_PROP(isptr p). {
+          entailer!.
+      }
+        rewrite HRE in H6.
+        simpl in H6.
+        contradiction.
+      }
+    }
+    rewrite H6 in H5.
+    simpl in H5.
+    forward. (* Over return *)
+    entailer!.
+    {
+      unfold hashtable_get.
+      rewrite Zlength_map.
+      rewrite H1.
+      rewrite <- H5.
+      reflexivity.
+    }
+    unfold hashtable_rep.
+    Exists bl.
+    entailer!.
+    remember (hashfun sigma mod 109) as bk.
+    remember (listrep [] nullval) as nl.
+    remember (listrep (Znth bk (map fst bl)) (Znth bk (map snd bl))) as Q.
+    sep_apply (modus_ponens_wand nl Q).
+    subst nl Q.
+    rewrite (iter_sepcon_split3 bk bl (uncurry listrep)) by auto.
+    cancel.
+    unfold uncurry.
+    repeat rewrite Znth_map by auto.
+    auto.
+  }
+
+}
+
+Qed.
+
+(** [] *)
+
+(** **** Exercise: 3 stars (listboxrep_traverse)  *)
+Lemma listboxrep_traverse:
+  forall p kp key count r,
+          field_compatible tcell [] p ->
+            cstring Tsh key kp *
+            field_at Tsh tcell [StructField _key] kp p *
+            field_at Tsh tcell [StructField _count] (Vint (Int.repr count)) p *
+            malloc_token Tsh tcell p *
+            data_at Tsh (tptr tcell) p r |--
+            ALL dl: list (string * Z),
+              listboxrep dl (field_address tcell [StructField _next] p)
+                -* listboxrep ((key, count) :: dl) r.
+Proof.
+  intros.
+  apply allp_right; intro dl.
+  apply -> wand_sepcon_adjoint.
+   (** Sometime during the proof below, you will have
+       [data_at Tsh tcell ... p]
+     that you want to expand into
+
+       field_at Tsh tcell [StructField _key] ... p
+     * field_at Tsh tcell [StructField _count] ... p
+     * field_at Tsh tcell [StructField _next] ... p].
+
+   You can do this with   [unfold_data_at x%nat] where x is the number
+   indicating _which_ of the [data_at] or [field_at] conjucts you want to expand.
+*)
+
+  unfold listboxrep.
+  Intros p'.
+  remember (field_address tcell [StructField _next] p) as y.
+  Exists p.
+  simpl (listrep ((key, count) :: dl) p).
+  Exists p'.
+  unfold list_cell.
+  Exists kp.
+  unfold_data_at 4%nat.
+  entailer!.
+  rewrite field_at_data_at.
+  entailer!.
+Qed.
+
+(** [] *)
+
+(** **** Exercise: 2 stars (body_incr_list)  *)
+
+Lemma incr_list_no_key:
+  forall (key: string) (al: list (string * Z)),
+    ~ (In key (map fst al)) -> (list_incr key al) = al ++ [(key, 1)].
+Proof.
+  intros key al.
+  induction al as [| [lhk lhc] lt]; intros.
+  { (* al is nil *)
+    reflexivity.
+  }
+  { (* al is (lhk, lhc) :: lt *)
+    simpl.
+    simpl in H.
+    destruct (EqDec_string key lhk).
+    { (* key = lhk *)
+      exfalso.
+      apply H.
+      left.
+      auto.
+    }
+    { (* key <> lhk *)
+      f_equal.
+      apply IHlt.
+      intro.
+      apply H.
+      right.
+      auto.
+    }
+  }
+Qed.
+
+Lemma incr_list_with_key:
+  forall (key: string) (al post: list (string * Z)) (count: Z),
+    ~ (In key (map fst al)) ->
+    (list_incr key (al ++ [(key, count)] ++ post)) = (al ++ [(key, count + 1)] ++ post).
+Proof.
+  intros key al.
+  induction al as [| [lhk lhc] lt]; intros.
+  { (* al is nil *)
+    simpl.
+    rewrite pred_dec_true by auto.
+    reflexivity.
+  }
+  { (* al is (lhk, lhc) :: lt *)
+    simpl.
+    simpl in H.
+    destruct (EqDec_string key lhk).
+    { (* key = lhk *)
+      exfalso.
+      apply H.
+      left.
+      auto.
+    }
+    { (* key <> lhk *)
+      f_equal.
+      apply IHlt.
+      intro.
+      apply H.
+      right.
+      auto.
+    }
+  }
+
+Qed.
+
+Definition partial_listbox_rep(P: (list (string * Z)) -> (list (string * Z)))
+           (r i: val) : mpred :=
+  ALL l: list (string * Z), ((listboxrep l i) -* (listboxrep (P l) r)).
+
+Lemma ptbr3a:
+  forall q p kp key count,
+    ((data_at Tsh (tptr tcell) p q) *
+     field_at Tsh tcell [StructField _key] kp p *
+     field_at Tsh tcell [StructField _count] (Vint (Int.repr count)) p *
+     cstring Tsh key kp *
+     malloc_token Tsh tcell p
+    )
+      |-- (partial_listbox_rep (fun l => (key, count) :: l) q
+                               (field_address tcell [StructField _next] p)).
+Proof.
+  intros.
+  unfold partial_listbox_rep.
+  apply allp_right.
+  intro v.
+  rewrite <- wand_sepcon_adjoint.
+  unfold listboxrep at 2.
+  Exists p.
+  unfold listrep.
+  unfold listboxrep.
+  Intros y.
+  Exists y.
+  fold (listrep v y).
+  unfold list_cell.
+  Exists kp.
+  cancel.
+  unfold_data_at 2%nat.
+  cancel.
+  rewrite field_at_data_at.
+  simpl.
+  unfold tcell.
+  auto.
+Qed.
+
+Lemma ptbr3c:
+  forall p,
+    emp |-- partial_listbox_rep (fun l => l) p p.
+Proof.
+  intros.
+  unfold partial_listbox_rep.
+  apply allp_right.
+  intro v.
+  apply wand_refl_cancel_right.
+Qed.
+
+Lemma ptbr3d:
+  forall t i r P,
+  ((listboxrep t i) * (partial_listbox_rep P r i))
+    |-- (listboxrep (P t) r).
+Proof.
+  intros.
+  unfold partial_listbox_rep.
+  rewrite sepcon_comm.
+  apply wand_sepcon_adjoint.
+  apply (allp_instantiate
+           (fun l : list (string * Z) => listboxrep l i -* listboxrep (P l) r)
+           t).
+Qed.
+
+Lemma ptbr3e:
+  forall P1 P2 p1 p2 p3,
+    (partial_listbox_rep P1 p2 p1) *
+    (partial_listbox_rep P2 p3 p2)
+      |-- (partial_listbox_rep
+             (fun l: list (string * Z) => (P2 (P1 l)))
+             p3 p1).
+Proof.
+  intros.
+  unfold partial_listbox_rep.
+  apply allp_right.
+  intro v.
+  assert((ALL l : list (string * Z) , listboxrep l p1 -* listboxrep (P1 l) p2)
+           |-- (listboxrep v p1 -* listboxrep (P1 v) p2)). {
+    apply (allp_instantiate
+             (fun l : list (string * Z) => listboxrep l p1 -* listboxrep (P1 l) p2)
+             v).
+  }
+  sep_apply H; clear H.
+  assert((ALL l : list (string * Z) , listboxrep l p2 -* listboxrep (P2 l) p3)
+           |-- listboxrep (P1 v) p2 -* listboxrep (P2 (P1 v)) p3). {
+    apply (allp_instantiate
+             (fun l : list (string * Z) => listboxrep l p2 -* listboxrep (P2 l) p3)
+             (P1 v)).
+  }
+  sep_apply H; clear H.
+  rewrite <- wand_sepcon_adjoint.
+  sep_apply (modus_ponens_wand (listboxrep v p1) (listboxrep (P1 v) p2)).
+  sep_apply (modus_ponens_wand (listboxrep (P1 v) p2) (listboxrep (P2 (P1 v)) p3)).
+  auto.
+Qed.
+
+Lemma listboxrep_fold:
+  forall p r al,
+    data_at Tsh (tptr tcell) p r * listrep al p |-- listboxrep al r.
+Proof.
+  intros.
+  unfold listboxrep.
+  Exists p.
+  cancel.
+Qed.
+
+Lemma hashtable_rep_fold: forall (p: val) (bl: list (list (string * Z) * val)),
+    malloc_token Tsh thashtable p *
+    field_at Tsh thashtable [StructField _buckets] (map snd bl) p *
+    iter_sepcon (uncurry listrep) bl
+                |-- hashtable_rep (map fst bl) p.
+Proof.
+  intros.
+  unfold hashtable_rep.
+  Exists bl.
+  entailer!.
+Qed.
+
+Lemma field_at_data_at':
+      forall {cs: compspecs} (sh : Share.t) (t : type) (gfs : list gfield)
+         (v : reptype (nested_field_type t gfs))
+         (p : val),
+       field_at sh t gfs v p =
+       !! field_compatible t gfs p  && data_at sh (nested_field_type t gfs) v (field_address t gfs p).
+Proof.
+intros.
+apply pred_ext.
+entailer!. rewrite field_at_data_at; auto.
+entailer!. rewrite field_at_data_at; auto.
+Qed.
+
+Lemma add1_rep:
+  forall x: Z,
+    (Int.add (Int.repr x) (Int.repr 1)) = Int.repr (x + 1).
+Proof.
+  intros.
+  unfold Int.add.
+  Search ((_ + _) mod _).
+  apply int_rep_helper.
+  rewrite !Int.unsigned_repr_eq.
+  remember Int.modulus as m.
+  rewrite <- Zplus_mod.
+  auto.
+Qed.
+
+Definition prepend_key_count (P: (list (string * Z)) -> (list (string * Z)))
+           (key: string) (count : Z) (l: list (string * Z)) :=
+    P((key, count) :: l).
+
+Lemma list_rep_listbox_rep: forall (t: list (string * Z)) (p : val),
+    listrep t p =
+    match t with
+    | [] => !!(p = nullval) && emp
+    | (s, c) :: tl => (EX kp: val,
+      malloc_token Tsh tcell p *
+      cstring Tsh s kp *
+      field_at Tsh tcell [StructField _key] kp p *
+      field_at Tsh tcell [StructField _count] (Vint (Int.repr c)) p *
+      listboxrep tl (field_address tcell [StructField _next] p))
+    end.
+Proof.
+  intros.
+  destruct t as [| [s c] tl]; auto.
+  unfold listboxrep; simpl.
+  apply pred_ext.
+  {
+    Intros y.
+    unfold list_cell.
+    Intros kp.
+    Exists kp.
+    entailer!.
+    unfold_data_at 1%nat.
+    Exists y.
+    cancel.
+    rewrite !field_at_data_at.
+    cancel.
+  }
+  {
+    Intros kp p0.
+    Exists p0.
+    unfold list_cell.
+    Exists kp.
+    entailer!.
+    unfold_data_at 2%nat.
+    rewrite !field_at_data_at.
+    cancel.
+  }
+Qed.
+
+Lemma listboxrep_spec: forall (t: list (string * Z)) (b: val),
+  listboxrep t b =
+  EX p: val,
+  data_at Tsh (tptr tcell) p b *
+    match t with
+    | [] => !!(p = nullval) && emp
+    | (s, c) :: tl => (EX kp: val,
+      malloc_token Tsh tcell p *
+      cstring Tsh s kp *
+      field_at Tsh tcell [StructField _key] kp p *
+      field_at Tsh tcell [StructField _count] (Vint (Int.repr c)) p *
+      listboxrep tl (field_address tcell [StructField _next] p))
+    end.
+Proof.
+  intros.
+  unfold listboxrep at 1.
+  f_equal.
+  extensionality p.
+  destruct t as [| [s c] tl]; simpl.
+  { apply pred_ext; entailer!. }
+  { (* Non-nil case *)
+    apply pred_ext; entailer!.
+    {
+      unfold list_cell.
+      Intros kp. Exists kp.
+      unfold_data_at 2%nat.
+      cancel.
+      unfold listboxrep.
+      Exists y.
+      cancel.
+      rewrite field_at_data_at.
+      cancel.
+    }
+    {
+      unfold listboxrep.
+      Intros q.
+      Exists q.
+      cancel.
+      unfold list_cell.
+      Exists kp.
+      cancel.
+      unfold_data_at 2%nat.
+      cancel.
+      rewrite field_at_data_at.
+      cancel.
+    }
+  }
+Qed.
+
+Lemma listboxrep_internal: forall b p kp s c tl,
+  data_at Tsh (tptr tcell) p b *
+  malloc_token Tsh tcell p *
+  cstring Tsh s kp *
+  field_at Tsh tcell [StructField _key] kp p *
+  field_at Tsh tcell [StructField _count] (Vint (Int.repr c)) p *
+  listboxrep tl (field_address tcell [StructField _next] p) |--
+  listboxrep ((s, c) :: tl) b.
+Proof.
+  intros.
+  rewrite (listboxrep_spec (cons _ _ )).
+  Exists p kp.
+  entailer!.
+Qed.
+
+Lemma body_incr_list: semax_body Vprog Gprog f_incr_list incr_list_spec.
+Proof.
+(** This proof uses "magic wand as frame" to traverse _and update_
+   a (linked list) data structure.   This pattern is a bit more complex than
+   the wand-as-frame pattern used in body_get, which did not update
+   the data structure.   You will still use "data-structure-with-a-hole"
+   and "what-is-in-the-hole"; but now the "data-structure-with-a-hole"
+   must be able to accept the _future_ hole-filler, not the one that is
+   in the hole right now.
+
+  The key lemmas to use are, [wand_refl_cancel_right], [wand_frame_elim'],
+   and [wand_frame_ver].   When using [wand_frame_ver], you will find
+   [listboxrep_traverse] to be useful.
+*)
+  start_function.
+  forward.
+  rename al into al0.
+  forward_loop
+    (EX P: (list (string * Z)) -> (list (string * Z)),
+           (EX r: val, (EX al: list (string * Z),
+       (PROP (
+            P(list_incr sigma al) = list_incr sigma al0;
+            (list_get sigma al0) = (list_get sigma al)
+          )
+        LOCAL (
+          temp _r r;
+          temp _s s
+        )
+        SEP (
+          listboxrep al r;
+          partial_listbox_rep P r0 r;
+          cstring Tsh sigma s
+        )
+    )))).
+  { (* Pre implies loop invariant *)
+    Exists (fun l: (list (string * Z)) => l).
+    Exists r0.
+    Exists al0.
+    entailer!.
+    apply ptbr3c.
+  }
+  { (* In body of loop *)
+    Intros P r al.
+    unfold listboxrep.
+    Intros p.
+    forward.
+    forward_if (p <> nullval).
+    { (* True branch *)
+      assert_PROP(al = []). {
+        entailer!.
+        apply H5;reflexivity.
+      }
+      subst al.
+      simpl in H0.
+      forward_call (s, sigma, 1, nullval).
+      Intros new_cell_ret.
+      forward.
+      sep_apply (listrep_fold_nil sigma 1 new_cell_ret).
+      sep_apply (listboxrep_fold new_cell_ret r [(sigma, 1)]).
+      sep_apply (ptbr3d [(sigma, 1)] r r0 P).
+      rewrite H0.
+      forward.
+    }
+    { (* False branch *)
+      forward.
+      entailer!.
+    }
+    (* After first if. *)
+    assert_PROP(p <> nullval). {
+      entailer!.
+    }
+    destruct al as [| [key' count'] lt]; rewrite list_rep_listbox_rep.
+    { (* al is nil, a contradiction *)
+      normalize.
+    }
+    { (* al is (key', count') :: lt *)
+      Intros kp. clear H2.
+      forward. (* temp = p-> key *)
+      forward_call (kp, key', s, sigma).
+      Intros strcmp_ret.
+      forward_if.
+      { (* True branch *)
+        subst strcmp_ret.
+        rewrite pred_dec_true in H2 by auto.
+        subst key'.
+        simpl in H0.
+        rewrite pred_dec_true in H0 by auto.
+        simpl in H1.
+        rewrite pred_dec_true in H1 by auto.
+        rewrite H1 in H. clear H1.
+        forward.
+        forward.
+        rewrite (add1_rep count').
+        sep_apply (listboxrep_internal r p kp sigma (count' + 1) lt).
+        forward.
+        cancel.
+        rewrite <- H0.
+        apply ptbr3d.
+      }
+      { (* False branch, key did not compare *)
+        forward.
+        rewrite pred_dec_false in H2 by auto.
+        simpl in H0.
+        rewrite pred_dec_false in H0 by auto.
+        Exists (fun l => P((key', count') :: l)).
+        Exists (field_address tcell [StructField _next] p).
+        Exists lt.
+        entailer!.
+        {
+          simpl in H1.
+          rewrite pred_dec_false in H1 by auto.
+          auto.
+        }
+        {
+          sep_apply (ptbr3a r p kp key' count').
+          apply ptbr3e.
+        }
+      }
+    }
+  }
+
+Qed.
+
+(** [] *)
+
+
+
+(** Examine this carefully: *)
+Check wand_slice_array.
+(*  : forall (lo hi n : Z) (t : type) (sh : Share.t)
+             (al' : list (reptype t)) (p : val),
+       0 <= lo <= hi ->
+       hi <= n ->
+       Zlength al' = n ->
+       data_at sh (tarray t n) al' p =
+       !! field_compatible (tarray (tptr tcell) n) [] p &&
+       data_at sh (tarray t (hi - lo))
+         (sublist lo hi al')
+         (field_address0 (tarray t n) [ArraySubsc lo] p) *
+       array_with_hole sh t lo hi n al p.
+*)
+(** Here (array_with_hole sh t lo hi n al p) means *)
+(*  :  (ALL cl : list (reptype t) ,
+         data_at sh (tarray t (hi - lo)) cl
+           (field_address0 (tarray t n) [ArraySubsc lo] p) -*
+         data_at sh (tarray t n)
+           (sublist 0 lo al' ++ cl ++ sublist hi n al') p)
+*)
+
+Lemma wand_slice_array_fold:
+  forall {cs: compspecs} lo hi n sh t (al: list (reptype t)) p,
+    0 <= lo <= hi ->
+    hi <= n ->
+    Zlength al = n ->
+    (field_compatible (tarray t n) nil p) ->
+  data_at sh (tarray t (hi-lo)) (sublist lo hi al) (field_address0 (tarray t n) (ArraySubsc lo :: nil) p) *
+  array_with_hole sh t lo hi n al p |--
+                  data_at sh (tarray t n) al p.
+Proof.
+  intros.
+  unfold array_with_hole.
+  entailer!.
+  allp_left (sublist lo hi al).
+  rewrite sepcon_comm.
+  sep_apply (wand_frame_elim (data_at sh (tarray t (hi - lo)) (sublist lo hi al) (field_address0 (tarray t (Zlength al)) [ArraySubsc lo] p))
+                             (data_at sh (tarray t (Zlength al)) (sublist 0 lo al ++ sublist lo hi al ++ sublist hi (Zlength al) al) p)).
+  rewrite app_assoc.
+  rewrite (sublist_rejoin 0 lo hi al) by omega.
+  rewrite (sublist_rejoin 0 hi (Zlength al) al) by omega.
+  rewrite sublist_same by auto.
+  auto.
+Qed.
+
+Lemma wand_slice_array_fold1:
+  forall {cs: compspecs} h n sh t (al: list (reptype t)) p,
+    0 <= h ->
+    (h+1) <= n ->
+    Zlength al = n ->
+    (field_compatible (tarray t n) nil p) ->
+  data_at sh (tarray t ((h+1) - h)) (sublist h (h+1) al) (field_address0 (tarray t n) (ArraySubsc h :: nil) p) *
+  array_with_hole sh t h (h+1) n al p |--
+                  data_at sh (tarray t n) al p.
+Proof.
+  intros.
+  sep_apply((wand_slice_array_fold h (h+1) n sh t al p)).
+  all: auto.
+  omega.
+Qed.
+
+
+(** **** Exercise: 4 stars (body_incr)  *)
+Lemma body_incr: semax_body Vprog Gprog f_incr incr_spec.
+Proof.
+start_function.
+rename p into table.
+rename H into Hmax.
+assert_PROP (isptr table) as Htable by entailer!.
+
+(** The next two lines would not be part of an ordinary Verifiable C proof,
+   they are here only to guide you through the bigger proof. *)
+match goal with
+  |- semax _ _ (Ssequence (Ssequence ?c1 (Ssequence ?c2 ?c3)) ?c4) _ =>
+  apply (semax_unfold_seq (Ssequence (Ssequence c1 c2) (Ssequence c3 c4))); [ reflexivity | ]
+end.
+pose (j :=
+          EX cts: list (list (string * Z) * val),
+                  PROP (contents = map fst cts;
+                        0 <= hashfun sigma mod N < N;
+                        Zlength cts = N)
+                  LOCAL (temp _b (Vint (Int.repr (hashfun sigma mod N)));
+                         temp _h (Vint (Int.repr (hashfun sigma)));
+                         temp _table table; temp _s s)
+                  SEP (cstring Tsh sigma s;
+                       malloc_token Tsh thashtable table;
+                       data_at Tsh (tarray (tptr tcell) N) (map snd cts) (field_address thashtable [StructField _buckets] table);
+                       iter_sepcon (uncurry listrep) cts)).
+apply semax_seq' with j;
+subst j;
+abbreviate_semax. {
+  forward_call (s, sigma). (* h = hash(s) *)
+  forward.
+  unfold hashtable_contents in *.
+  unfold hashtable_rep.
+  Intros bl.
+  Exists bl.
+  entailer!.
+  {
+    split; [split |].
+    {
+      rewrite N_eq.
+      apply Z.mod_pos_bound; omega.
+    }
+    {
+      simplify_value_fits in H2.
+      destruct H2.
+      rewrite Zlength_map in H.
+      rewrite N_eq; auto.
+    }
+    {
+      f_equal.
+      unfold Int.modu.
+      apply int_rep_helper.
+      rewrite !Int.unsigned_repr; try rep_omega.
+      Lemma hashfun_limit: forall str,
+          0 <= hashfun str <= Int.max_unsigned.
+      Proof.
+        intros.
+        unfold hashfun.
+        rewrite hashfun_aux_equiv''.
+        unfold hashfun_aux''.
+        remember (rev str) as rs.
+        destruct rs; simpl.
+        {
+          rep_omega.
+        }
+        {
+          unfold hash_step'; simpl.
+          generalize (fold_right (fun (c : byte) (hin : Z) => hash_step hin c) 0 rs).
+          intro z.
+          unfold hash_step.
+          unfold Int.max_unsigned.
+          generalize (z * 65599 + Byte.signed i); intros.
+          assert(forall a b: Z, 0 <= a < b ->  0 <= a <= b - 1). {
+            intros. omega.
+          }
+          apply H; clear H.
+          apply Z.mod_pos_bound; rep_omega.
+        }
+      Qed.
+      apply (hashfun_limit sigma).
+    }
+  }
+  {
+    rewrite field_at_data_at.
+    entailer!.
+  }
+}
+{
+  Intros cts.
+  rewrite H in Hmax.
+  assert_PROP(field_compatible thashtable [StructField _buckets] table). {
+    entailer!.
+  }
+  rename H2 into FCT.
+
+  unfold hashtable_get in Hmax.
+  rewrite Zlength_map, H1 in Hmax.
+  set (h := hashfun sigma mod N) in *.
+  remember (map snd cts) as bkptrs.
+  remember (field_address thashtable [StructField _buckets] table) as bucketsAdr.
+  rewrite (wand_slice_array h (h+1) N Tsh (tptr tcell) bkptrs bucketsAdr);
+    try rewrite Heqbkptrs; try rewrite Zlength_map; try rep_omega.
+
+(** For the remainder of the proof, here are some useful lemmas:
+    [sublist_len_1] [sublist_same] [sublist_map]
+    [data_at_singleton_array_eq]
+    [iter_sepcon_split3]  [iter_sepcon_app] [sublist_split]
+    [field_at_data_at]
+    [wand_slice_array_tptr_tcell]
+ *)
+  Intros.
+  assert(K: h + 1 - h = 1). {
+    omega.
+  }
+  rewrite K. clear K.
+  rewrite sublist_len_1; try rewrite Zlength_map; try rewrite H1; auto.
+  rewrite <- Heqbkptrs.
+  remember (field_address0 (tarray (tptr tcell) N) [ArraySubsc h] bucketsAdr) as bk.
+  rewrite (data_at_singleton_array_eq Tsh (tptr tcell) (Znth h bkptrs)).
+  rewrite (iter_sepcon_split3 h cts (uncurry listrep));repeat rewrite Zlength_map; repeat rewrite H1; auto.
+  unfold uncurry at 2.
+  rewrite <- !(Znth_map h fst);repeat rewrite Zlength_map; repeat rewrite H1; auto.
+  rewrite <- !(Znth_map h snd);repeat rewrite Zlength_map; repeat rewrite H1; auto.
+  rewrite <- Heqbkptrs in *.
+  rewrite <- H in *.
+  remember (Znth h bkptrs) as p.
+  remember (Znth h contents) as al.
+  sep_apply (listboxrep_fold p bk al).
+  forward_call (bk, al, s, sigma). (* incr_list (& table->buckets[b], s); *)
+  3: reflexivity.
+  {
+    entailer!.
+    f_equal.
+    assert(FAT: (field_address thashtable [StructField _buckets] table) = table). {
+      unfold field_address.
+      normalize.
+      destruct (field_compatible_dec thashtable [StructField _buckets] table).
+      {
+        reflexivity.
+      }
+      {
+        contradiction.
+      }
+    }
+    unfold field_address0.
+    destruct (field_compatible0_dec (tarray (tptr tcell) N) [ArraySubsc h] (field_address thashtable [StructField _buckets] table)).
+    { (* field compatible *)
+      simpl.
+      normalize.
+      rewrite FAT.
+      reflexivity.
+    }
+    unfold field_compatible0 in n.
+    exfalso.
+    apply n.
+    clear n.
+    rewrite FAT.
+    rewrite FAT in H2.
+    destruct H2 as [? A].
+    repeat destruct A as [? A].
+    repeat split;auto; try omega.
+  }
+  {
+    forward.
+    cancel.
+
+    unfold hashtable_rep.
+    unfold hashtable_incr.
+    rewrite Zlength_map in *.
+    rewrite H1 in *.
+    unfold h in *.
+    clear h.
+    remember (hashfun sigma mod N) as h.
+    remember (map fst cts) as old_contents.
+    remember (list_incr sigma (Znth h old_contents)) as B.
+    remember (field_address0 (tarray (tptr tcell) N) [ArraySubsc h] (field_address thashtable [StructField _buckets] table)) as Bp.
+    unfold listboxrep.
+    Intros p.
+    Exists (upd_Znth h cts (B, p)).
+    rewrite <- upd_Znth_map.
+    simpl.
+    rewrite <- Heqold_contents.
+    simpl.
+    normalize.
+    cancel.
+    rewrite (iter_sepcon_split3 h (upd_Znth h cts (B, p)) (uncurry listrep)).
+    rewrite sublist_upd_Znth_l by omega.
+    rewrite sublist_upd_Znth_r; try omega.
+    cancel.
+    all: rewrite upd_Znth_Zlength.
+    all: rewrite H1.
+    all: rewrite N_eq in *.
+    cancel.
+    2-6: omega.
+    unfold uncurry.
+    remember (map snd cts) as old_bkps.
+    repeat rewrite upd_Znth_same by omega.
+    simpl.
+    rewrite <- (upd_Znth_map snd).
+    rewrite <- Heqold_bkps.
+    simpl.
+    unfold array_with_hole.
+    normalize.
+    hint.
+    autorewrite with sublist.
+    rewrite <- HeqBp.
+    repeat rewrite upd_Znth_same by omega.
+    simpl.
+    allp_left [p].
+    rewrite sepcon_comm.
+    rewrite (data_at_singleton_array_eq Tsh (tptr tcell) p) by auto.
+    sep_apply(wand_frame_elim (data_at Tsh (tptr tcell) p Bp)
+                              (data_at Tsh (tarray (tptr tcell) 109) (sublist 0 h old_bkps ++ [p] ++ sublist (h + 1) 109 old_bkps)
+                                       (field_address thashtable [StructField _buckets] table))).
+    assert(Zlength old_bkps = 109). {
+      subst old_bkps.
+      rewrite Zlength_map; auto.
+    }
+    assert((sublist 0 h old_bkps ++ [p] ++ sublist (h + 1) 109 old_bkps) =
+           (upd_Znth h old_bkps p)). {
+      rewrite <- (sublist_same 0 109 old_bkps) at 3 by omega.
+      rewrite (sublist_split 0 h 109 old_bkps) by omega.
+      rewrite (sublist_split h (h+1) 109 old_bkps) by omega.
+      rewrite (upd_Znth_app2 (sublist 0 h old_bkps)).
+      f_equal.
+      rewrite Zlength_sublist_correct.
+      assert(h - (h - 0) = 0). omega.
+      rewrite H6; clear H6.
+      rewrite upd_Znth0.
+      simpl.
+      f_equal.
+      autorewrite with sublist.
+      reflexivity.
+      omega.
+      omega.
+      rewrite Zlength_app.
+      repeat rewrite Zlength_sublist_correct by omega.
+      omega.
+    }
+    {
+      cancel.
+      rewrite field_at_data_at.
+      entailer!.
+    }
+  }
+}
+Qed.
+(** [] *)
