formal/task01/state_list_spec.v
@@ -1,0 +1,13 @@
+(** * Verif_hash: Correctness proof of hash.c *)
+
+Require Import VST.floyd.proofauto.
+Require Import VST.floyd.library.
+Require Import  hash.
+Instance CompSpecs : compspecs. make_compspecs prog. Defined.
+Definition Vprog : varspecs.  mk_varspecs prog. Defined.
+
+Require Import VST.msl.wand_frame.
+Require Import VST.msl.iter_sepcon.
+Require Import VST.floyd.reassoc_seq.
+Require Import VST.floyd.field_at_wand.
+Require Import Hashfun.
