formal/theories/verif_digsim.v
@@ -1,0 +1,45 @@
+(* Verify simple double floating add. *)
+Require Import VST.floyd.proofauto.
+
+Record Model : Set :=
+  mkModel {
+
+      x : float;
+      xd : float
+    }.
+
+Record Driver : Set :=
+  mkDriver {
+      done : bool;
+      s : Model;
+      states : list (float -> Model -> Model)
+    }.
+
+Record Event : Set :=
+  mkEvent {
+      etime : float;
+      ename : string;
+      efunc : Driver -> Driver
+    }.
+
+Definition Events := list Event.
+
+Fixpoint merge (l1 l2 : events) :=
+  let fix merge_aux l2 :=
+  match l1, l2 with
+  | [], _ => l2
+  | _, [] => l1
+  | a1::l1', a2::l2' =>
+      if a1 <=? a2 then a1 :: merge l1' l2 else a2 :: merge_aux l2'
+  end
+  in merge_aux l2.
+
+Float.add
+Definition terminate (d: Driver) :=
+  {| done := true; s := d.(s); states := d.(states) |}.
+
+Section Test.
+
+End Test.
+
+
