formal/task01/build.sh
@@ -1,0 +1,11 @@
+#!/bin/bash
+if [ ! -d cmake-build-release ]
+then
+  mkdir cmake-build-release
+fi
+cd cmake-build-release
+
+cmake -DCMAKE_BUILD_TYPE=Release ..
+cmake --build  .
+
+cd ..
