formal/theories/Task01/README.md
@@ -1,0 +1,19 @@
+# c sources - digsim task01
+digsim task01 used in haskell equivalency tests 
+
+requires cmake >= 3.10 and clang >= 3.8
+
+build and plot
+```bash
+bash plot.sh
+```
+build
+```bash
+bash build.sh
+```
+
+run (after build)
+```bash
+./cmake-build-release/task01
+```
+
