formal/theories/Task01/plot.sh
@@ -1,0 +1,4 @@
+#!/usr/bin/env bash
+bash build.sh
+./cmake-build-release/task01
+gnuplot digsim.plt
